@prefix : <http://mmoon.org/mmoon/> .
@prefix dc: <http://purl.org/dc/elements/1.1/> .
@prefix owl: <http://www.w3.org/2002/07/owl#> .
@prefix rdf: <http://www.w3.org/1999/02/22-rdf-syntax-ns#> .
@prefix xml: <http://www.w3.org/XML/1998/namespace> .
@prefix xsd: <http://www.w3.org/2001/XMLSchema#> .
@prefix gold: <http://purl.org/linguistics/gold/> .
@prefix rdfs: <http://www.w3.org/2000/01/rdf-schema#> .
@prefix skos: <http://www.w3.org/2004/02/skos/core#> .
@prefix lexvo: <http://lexvo.org/ontology#> .
@prefix mmoon: <http://mmoon.org/mmoon/> .
@base <http://mmoon.org/mmoon/> .

<http://mmoon.org/mmoon/> rdf:type owl:Ontology ;
                          
                          rdfs:label "Multilingual Morpheme Ontology"@en ;
                          
                          rdfs:comment """The Multilingual Morpheme Ontology (MMoOn) is  an ontological model that contains the vocabulary needed to describe the morphological elements, meanings and representations of natural languages. 

This is the reference ontology from which various language specific MMoOn Inventories can be derived."""@en ;
                          
                          owl:versionInfo "Version 1.0, 2016"@en .


#################################################################
#
#    Annotation properties
#
#################################################################


###  http://mmoon.org/mmoon/definition

:definition rdf:type owl:AnnotationProperty ;
            
            rdfs:comment "A definition for MMoOn vocabulary item (classes, properties, also possibly individuals)."@en ;
            
            rdfs:subPropertyOf rdfs:comment ,
                               skos:definition .



###  http://mmoon.org/mmoon/example

:example rdf:type owl:AnnotationProperty ;
         
         rdfs:subPropertyOf rdfs:comment .



###  http://mmoon.org/mmoon/externalDefinition

:externalDefinition rdf:type owl:AnnotationProperty ;
                    
                    rdfs:comment """A reference to an (typically alternative) definition for MMoOn vocabulary items. 

Solely to be used to refer to Web Resources identified by their URI/IRI (which ideally should be Linked Data)."""@en ;
                    
                    rdfs:range rdfs:Resource ;
                    
                    rdfs:subPropertyOf rdfs:comment .



###  http://mmoon.org/mmoon/externalDefinitionDesc

:externalDefinitionDesc rdf:type owl:AnnotationProperty ;
                        
                        rdfs:comment """A reference to an (typically alternative) definition for MMoOn vocabulary items. 

To be used when no URI/IRI can be provided as
reference point or when additional textual information has to be provided for an URI/IRI reference to be sufficiently specific."""@en ;
                        
                        rdfs:subPropertyOf rdfs:comment ;
                        
                        rdfs:range xsd:string .



###  http://mmoon.org/mmoon/usageNote

:usageNote rdf:type owl:AnnotationProperty ;
           
           rdfs:subPropertyOf rdfs:comment .



###  http://www.w3.org/2004/02/skos/core#definition

skos:definition rdf:type owl:AnnotationProperty .





#################################################################
#
#    Object Properties
#
#################################################################


###  http://mmoon.org/mmoon/associatedToLanguage

:associatedToLanguage rdf:type owl:ObjectProperty ;
                      
                      rdfs:label "associated to language"@en ;
                      
                      rdfs:comment "States that a morpheme inventory, morph or word is associated to a specific langauge."@en ;
                      
                      rdfs:range lexvo:Language .



###  http://mmoon.org/mmoon/attachedToRoot

:attachedToRoot rdf:type owl:ObjectProperty ;
                
                rdfs:label "attached to root"@en ;
                
                rdfs:comment "States that an affix is attached to some root."@en ;
                
                rdfs:domain :Affix ;
                
                rdfs:range :Root .



###  http://mmoon.org/mmoon/attachedToStem

:attachedToStem rdf:type owl:ObjectProperty ;
                
                rdfs:label "attached to stem"@en ;
                
                rdfs:comment "States that an affix is attached to some stem."@en ;
                
                rdfs:domain :Affix ;
                
                rdfs:range :Stem .



###  http://mmoon.org/mmoon/belongsToLexeme

:belongsToLexeme rdf:type owl:ObjectProperty ;
                 
                 rdfs:label "belongs to lexeme"@en ;
                 
                 rdfs:comment "States that a word-form resource belongs to a lexeme resource."@en ;
                 
                 rdfs:range :Lexeme ;
                 
                 rdfs:domain :Wordform ;
                 
                 owl:inverseOf :hasWordform .



###  http://mmoon.org/mmoon/belongsToWord

:belongsToWord rdf:type owl:ObjectProperty ;
               
               rdfs:label "belongs to word"@en ;
               
               rdfs:comment "States that a morph belongs to some word."@en ;
               
               rdfs:domain :Morph ;
               
               rdfs:range :Word ;
               
               owl:inverseOf :consistsOfMorph .



###  http://mmoon.org/mmoon/compoundingRelation

:compoundingRelation rdf:type owl:ObjectProperty ;
                     
                     rdfs:label "States which kind of compounding morphological relationship applies to a compound word."@en ,
                                "compounding morphological relationship"@en ;
                     
                     rdfs:domain :CompoundWord ;
                     
                     rdfs:range :Compounding ;
                     
                     rdfs:subPropertyOf :hasMorphologicalRelationship .



###  http://mmoon.org/mmoon/consistsOfAffix

:consistsOfAffix rdf:type owl:ObjectProperty ;
                 
                 rdfs:label "consists of affix"@en ;
                 
                 rdfs:comment "States that a  word, stem or root consists of some affix."@en ;
                 
                 rdfs:range :Affix ;
                 
                 rdfs:subPropertyOf :consistsOfMorph ;
                 
                 rdfs:domain [ rdf:type owl:Class ;
                               owl:unionOf ( :Root
                                             :Stem
                                             :Word
                                           )
                             ] .



###  http://mmoon.org/mmoon/consistsOfMorph

:consistsOfMorph rdf:type owl:ObjectProperty ;
                 
                 rdfs:label "consists of morph"@en ;
                 
                 rdfs:comment "States that a word consists of some morph."@en ;
                 
                 rdfs:range :Morph ;
                 
                 rdfs:domain :Word .



###  http://mmoon.org/mmoon/consistsOfMorpheme

:consistsOfMorpheme rdf:type owl:ObjectProperty ;
                    
                    rdfs:label "States that a complex morpheme consists of fusional and/or atomic and/or empty morphemes."@en ,
                               "consist of morpheme"@en ;
                    
                    rdfs:domain :ComplexMorpheme ;
                    
                    rdfs:range [ rdf:type owl:Class ;
                                 owl:unionOf ( :AtomicMorpheme
                                               :EmptyMorpheme
                                               :FusionalMorpheme
                                             )
                               ] .



###  http://mmoon.org/mmoon/consistsOfRoot

:consistsOfRoot rdf:type owl:ObjectProperty ;
                
                rdfs:label "consists of root"@en ;
                
                rdfs:comment "States that a stem or word consists of some root."@en ;
                
                rdfs:range :Root ;
                
                rdfs:subPropertyOf :consistsOfMorph ;
                
                rdfs:domain [ rdf:type owl:Class ;
                              owl:unionOf ( :Stem
                                            :Word
                                          )
                            ] .



###  http://mmoon.org/mmoon/consistsOfStem

:consistsOfStem rdf:type owl:ObjectProperty ;
                
                rdfs:label "consists of stem"@en ;
                
                rdfs:comment "States that a word or stem consists of some stem."@en ;
                
                rdfs:range :Stem ;
                
                rdfs:subPropertyOf :consistsOfMorph ;
                
                rdfs:domain [ rdf:type owl:Class ;
                              owl:unionOf ( :Stem
                                            :Word
                                          )
                            ] .



###  http://mmoon.org/mmoon/consistsOfWord

:consistsOfWord rdf:type owl:ObjectProperty ;
                
                rdfs:label "consists of word"@en ;
                
                rdfs:comment "States that an analytic word-form (such as \"more big\" being the comparative form of the adjective \"big\") consists of other word resources."@en ;
                
                rdfs:domain :AnalyticWordform ;
                
                rdfs:range :Word .



###  http://mmoon.org/mmoon/correspondsToMorpheme

:correspondsToMorpheme rdf:type owl:ObjectProperty ;
                       
                       rdfs:label "corresponds to morpheme"@en ;
                       
                       rdfs:comment "States that a given morph corresponds to a certain morpheme."@en ;
                       
                       rdfs:domain :Morph ;
                       
                       rdfs:range :Morpheme .



###  http://mmoon.org/mmoon/derivationalRelation

:derivationalRelation rdf:type owl:ObjectProperty ;
                      
                      rdfs:label "States which kind of derivational morphological relationship applies to a derived word."@en ,
                                 "derivational morphological relationship"@en ;
                      
                      :usageNote "This property is also used to state that a simple lexeme which cannot be further segmented with respect to word-formation has the morphological relationship mmoon:NoWordFormation."@en ;
                      
                      rdfs:range :Derivation ;
                      
                      rdfs:domain :DerivedWord ;
                      
                      rdfs:subPropertyOf :hasMorphologicalRelationship .



###  http://mmoon.org/mmoon/forLanguage

:forLanguage rdf:type owl:ObjectProperty ;
             
             rdfs:label "for language"@en ;
             
             rdfs:comment "States that a MMoOn morpheme inventory is specified for a certain language."@en ;
             
             rdfs:domain :MorphemeInventory ;
             
             rdfs:subPropertyOf :associatedToLanguage .



###  http://mmoon.org/mmoon/hasMeaning

:hasMeaning rdf:type owl:ObjectProperty ;
            
            rdfs:label "has meaning"@en ;
            
            rdfs:range :Meaning ;
            
            rdfs:domain [ rdf:type owl:Class ;
                          owl:unionOf ( :Morpheme
                                        :Word
                                      )
                        ] .



###  http://mmoon.org/mmoon/hasMorphemicEntry

:hasMorphemicEntry rdf:type owl:ObjectProperty ;
                   
                   rdfs:label "has morphemic entry"@en ;
                   
                   rdfs:comment "States that a morpheme inventory resource has morphemes as morphemic entries, thus building the intension of the morpheme inventory."@en ;
                   
                   rdfs:range :Morpheme ;
                   
                   rdfs:domain :MorphemeInventory .



###  http://mmoon.org/mmoon/hasMorphologicalRelationship

:hasMorphologicalRelationship rdf:type owl:ObjectProperty ;
                              
                              rdfs:label "has morphological relationship"@en ;
                              
                              rdfs:comment "Specifies the morphological relationship of a word."@en ;
                              
                              rdfs:range :MorphologicalRelationship ;
                              
                              rdfs:domain :Word .



###  http://mmoon.org/mmoon/hasRealization

:hasRealization rdf:type owl:ObjectProperty ;
                
                rdfs:label "has realization"@en ;
                
                rdfs:comment "States that a morpheme is realized by some morph."@en ;
                
                rdfs:range :Morph ;
                
                rdfs:domain :Morpheme ;
                
                owl:inverseOf :correspondsToMorpheme .



###  http://mmoon.org/mmoon/hasRepresentation

:hasRepresentation rdf:type owl:ObjectProperty ;
                   
                   rdfs:label "has representation"@en ;
                   
                   rdfs:range :Representation ;
                   
                   rdfs:domain [ rdf:type owl:Class ;
                                 owl:unionOf ( :Morph
                                               :Word
                                             )
                               ] .



###  http://mmoon.org/mmoon/hasWordform

:hasWordform rdf:type owl:ObjectProperty ;
             
             rdfs:label "has wordform"@en ;
             
             rdfs:comment "States that (typically) a lexeme resource has an associated word-form resource."@en ;
             
             rdfs:range :Wordform ;
             
             rdfs:domain [ rdf:type owl:Class ;
                           owl:unionOf ( :GrammaticalWord
                                         :Lexeme
                                       )
                         ] .



###  http://mmoon.org/mmoon/inflectionalRelation

:inflectionalRelation rdf:type owl:ObjectProperty ;
                      
                      rdfs:label "States which kind of inflectional morphological relationship applies to a word-form."@en ,
                                 "inflectional morphological relationship"@en ;
                      
                      rdfs:range :Inflection ;
                      
                      rdfs:domain :Wordform ;
                      
                      rdfs:subPropertyOf :hasMorphologicalRelationship .



###  http://mmoon.org/mmoon/isAllomorphTo

:isAllomorphTo rdf:type owl:ObjectProperty ,
                        owl:SymmetricProperty ;
               
               rdfs:label "is allomorph to"@en ;
               
               rdfs:comment "States that a morph is an allomorph to another morph which are both realizations of the same morpheme and which occur in complementary or free distribution."@en ;
               
               rdfs:seeAlso """http://www-01.sil.org/linguistics/GlossaryOflinguisticTerms/WhatIsAnAllomorph.htm: 
An allomorph is one of two or more complementary morphs which manifest a morpheme in its different phonological or morphological environments."""@en ;
               
               rdfs:range :Morph ;
               
               rdfs:domain :Morph .



###  http://mmoon.org/mmoon/isComposedOf

:isComposedOf rdf:type owl:ObjectProperty ;
              
              rdfs:label "is composed of"@en ;
              
              rdfs:comment "States of which lexemes or grammatical words the compound word is composed."@en ;
              
              rdfs:domain :CompoundWord ;
              
              rdfs:range [ rdf:type owl:Class ;
                           owl:unionOf ( :GrammaticalWord
                                         :Lexeme
                                       )
                         ] .



###  http://mmoon.org/mmoon/isDerivedFrom

:isDerivedFrom rdf:type owl:ObjectProperty ;
               
               rdfs:label "States from which lexeme or grammatical word the derived word is derived."@en ,
                          "is derived from"@en ;
               
               rdfs:domain :DerivedWord ;
               
               rdfs:range [ rdf:type owl:Class ;
                            owl:unionOf ( :GrammaticalWord
                                          :Lexeme
                                        )
                          ] .



###  http://mmoon.org/mmoon/isHomonymTo

:isHomonymTo rdf:type owl:ObjectProperty ,
                      owl:SymmetricProperty ;
             
             rdfs:label "is homonym to"@en ;
             
             rdfs:comment "States that a morph is homonym to another morph, i.e. although sharing the same orthographic and/or morphemic representation both morphs encode different meanings and thus realize different morphemes."@en ;
             
             rdfs:range :Morph ;
             
             rdfs:domain :Morph .



###  http://mmoon.org/mmoon/partOfLanguage

:partOfLanguage rdf:type owl:ObjectProperty ;
                
                rdfs:label "part of language"@en ;
                
                rdfs:comment "States that a morph or word resources is a linguistic entity as part of a certain language."@en ;
                
                rdfs:subPropertyOf :associatedToLanguage ;
                
                rdfs:domain [ rdf:type owl:Class ;
                              owl:unionOf ( :Morph
                                            :Word
                                          )
                            ] .





#################################################################
#
#    Data properties
#
#################################################################


###  http://mmoon.org/mmoon/morphemicRepresentation

:morphemicRepresentation rdf:type owl:DatatypeProperty ;
                         
                         rdfs:label "morphemic representation"@en ;
                         
                         rdfs:comment """The morphemic representation of a morph.
It includes:
a) marking of the prefix  boundary with a hyphen, eg. prefix-
b) marking of the suffix boundary with a hyphen, e.g. -suffix
c) marking of the infix boundry inclosed in angled brackets, e.g. <infix>
d) marking of the circumfix boundary by setting them off by angled brackets, e.g. circumfix prefix><circumfix suffix
e) marking of the transfix and simulfix boundary with a backslash, e.g. \\transfix or simulfix
g) marking of the zero morph and empty morph according to the position they take, e.g. in prefix position: zero/empty morph- , in suffix position: -zero/empty morph

The morphemic representation consists of a morphemic boundary marking and the conventional orthographic representation of it. It differs from the orthographic representation in that it is marked by one of the typographic conventions a) - g). It differs from the morphemic gloss in that it renders the orthographic representation of the morph instead of the corresponding meaning glosses. I.e. for the English genetive \"-s\" morph the three representations are as follows:

orthographic rep.: \"s\"
morphemic rep.: \"-s\"
morphemic gloss: \"GEN\""""@en ;
                         
                         rdfs:domain :Representation ;
                         
                         rdfs:range xsd:string .



###  http://mmoon.org/mmoon/orthographicRepresentation

:orthographicRepresentation rdf:type owl:DatatypeProperty ;
                            
                            rdfs:label "orthographic representation"@en ;
                            
                            rdfs:comment "Is the representation adhering to the charactersof the writing system (graphemes) according to the language of the MMoOn inventory."@en ;
                            
                            rdfs:domain :Representation ;
                            
                            rdfs:range xsd:string .



###  http://mmoon.org/mmoon/phoneticRepresentation

:phoneticRepresentation rdf:type owl:DatatypeProperty ;
                        
                        rdfs:label "phonetic representation"@en ;
                        
                        rdfs:comment "Is the phonetic representation according to the IPA. symbols."@en ;
                        
                        rdfs:domain :Representation ;
                        
                        rdfs:range xsd:string .



###  http://mmoon.org/mmoon/transliteration

:transliteration rdf:type owl:DatatypeProperty ;
                 
                 rdfs:label "transliteration"@en ;
                 
                 :usageNote "A reference to the mapping relation of the two writing system involved is highly recommended."@en ;
                 
                 rdfs:comment "This property renders orthographic representations of the writing system of the language of the morpheme inventory in symbols of another writing system, which ideally adheres to the latin alphabet."@en ;
                 
                 rdfs:seeAlso <https://en.wikipedia.org/wiki/ISO_basic_Latin_alphabet> .





#################################################################
#
#    Classes
#
#################################################################


###  http://lexvo.org/ontology#Language

lexvo:Language rdf:type owl:Class ;
               
               rdfs:label "Language"@en ;
               
               rdfs:isDefinedBy "http://lexvo.org/ontology#Language"@en .



###  http://mmoon.org/mmoon/ActionNoun

:ActionNoun rdf:type owl:Class ;
            
            rdfs:label "Action noun"@en ;
            
            rdfs:subClassOf :DeverbalNoun ;
            
            rdfs:comment "A noun which is derived from a verb stem denoting the action of the deriving verb stem."@en ;
            
            rdfs:seeAlso """Christian Lehmann, under \"action noun\" at http://linguistik.uni-erfurt.de:8080/lido/Lido :
An action noun is a non-oriented verbal noun (nomen substantivum), i.e. one which designates the same kind of thing as a (finite) verb, viz. a situation core, except that this is hypostatized as an entity. An action noun is a non-oriented verbal noun (nomen substantivum), i.e. one which designates the same kind of thing as a (finite) verb, viz. a situation core, except that this is hypostatized as an entity."""@en ;
            
            :example "Eng. \"to arrive\"(V) --> \"arrival\"(N)."@en .



###  http://mmoon.org/mmoon/AdjectivalInflection

:AdjectivalInflection rdf:type owl:Class ;
                      
                      rdfs:label "Adjectival inflection"@en ;
                      
                      rdfs:subClassOf :Inflection ;
                      
                      rdfs:comment "Is the process of generating word-forms of adjectival stems."@en .



###  http://mmoon.org/mmoon/AdjectiveCompound

:AdjectiveCompound rdf:type owl:Class ;
                   
                   rdfs:label "Adjective compound"@en ;
                   
                   rdfs:subClassOf :Compounding ;
                   
                   rdfs:comment "An adjective compound is an adjective formed by composition of an adjective stem and another stem."@en ;
                   
                   :example "Eng.: \"man-eating\"(Adj) = \"man\"(N) + \"eating\"(Adj)."@en .



###  http://mmoon.org/mmoon/AdjectiveNoun

:AdjectiveNoun rdf:type owl:Class ;
               
               rdfs:label "Adjective noun"@en ;
               
               rdfs:subClassOf :Conversion ;
               
               rdfs:comment "An adjective noun is a noun which is fomed by conversion from an adjective and which entails no further derivational meaning except the entailed wordclass-change."@en ;
               
               :example "Engl.: \"old\"(Adj) --> \"the old\"(N)."@en .



###  http://mmoon.org/mmoon/AdjectiveVerb

:AdjectiveVerb rdf:type owl:Class ;
               
               rdfs:label "Adjective verb"@en ;
               
               rdfs:subClassOf :Conversion ;
               
               :example "German: \"dicht\"(Adj.) 'impermeable' --> \"dichten\"(V) 'seal'."@de ;
               
               rdfs:comment "An adjective verb is a verb which is fomed by conversion from an adjective and which entails no further derivational meaning except the entailed wordclass-change."@en .



###  http://mmoon.org/mmoon/AdverbCompound

:AdverbCompound rdf:type owl:Class ;
                
                rdfs:label "Adverb compound"@en ;
                
                rdfs:subClassOf :Compounding ;
                
                rdfs:comment "An adverb compound is an adverb formed by composition of an adverb stem and another stem."@en ;
                
                :example "Eng.: \"downstream\"(Adv) = \"down\"(Adv) + \"stream\"(N)."@en .



###  http://mmoon.org/mmoon/Affix

:Affix rdf:type owl:Class ;
       
       rdfs:label "Affix"@en ;
       
       owl:equivalentClass gold:Affix ;
       
       rdfs:subClassOf :Morph ;
       
       rdfs:comment "An affix is a bound segmental morph that is joined to a stem or root before, after, or within it, in the formation of a derived or inflected form. [Christian Lehmann, under \"affix\" at http://linguistik.uni-erfurt.de:8080/lido/Lido ]"@en .



###  http://mmoon.org/mmoon/AgentNoun

:AgentNoun rdf:type owl:Class ;
           
           rdfs:label "Agent noun"@en ;
           
           rdfs:subClassOf :DeverbalNoun ;
           
           rdfs:comment "A noun which is derived from a verb stem denoting someone or something that performs the action of the verb base."@en ;
           
           :example "Eng. \"to work\"(V) --> \"worker\"(N)."@en .



###  http://mmoon.org/mmoon/AnalyticWordform

:AnalyticWordform rdf:type owl:Class ;
                  
                  rdfs:label "Analytic word-form"@en ;
                  
                  rdfs:subClassOf :Wordform ;
                  
                  rdfs:comment """A word form is analytic iff it consists of more than one word form such that the lexical meaning provides the root of one of them, while the grammatical meaning components are coded in the other word forms (some of them possibly in the lexical word form).
An inflection is analytic to the extent that it consists of analytic word forms.

Delimitation and History:
’analytic’ is extensionally equivalent to ‚periphrastic’, but is also used to characterize a whole language type.
An analytic system has grammatical words; an isolating system does not.

Periphrastic conjugation is the formation of a verbal inflectional paradigm which consists of periphrastic forms.
Periphrastic conjugation is the formation of a verbal inflectional paradigm which consists of periphrastic forms.

Periphrasis is the combination of a grammatical word G with a lexical word L such that the result is equivalent to a morphological form of L inflected for the category of G.

Analytic Procedures:
Within one language, periphrasis is recognized by a paradigmatic relation between a periphrastic and a synthetic expression. Across languages or stages of one language, periphrasis in a looser sense is recognized on the basis of functional similarity. [Christian Lehmann, under \"analytic structure\" at http://linguistik.uni-erfurt.de:8080/lido/Lido]"""@en ;
                  
                  :example """The comparison of adjectives in English involves both inflectional forms (e.g. bigger) and periphrastic constructions (e.g. more interesting).
Engl. sang (synthetic) vs. has sung (periphrastic). [Christian Lehmann, under \"periphrasis\" at http://linguistik.uni-erfurt.de:8080/lido/Lido]"""@en .



###  http://mmoon.org/mmoon/ApplicativeVerb

:ApplicativeVerb rdf:type owl:Class ;
                 
                 rdfs:label "Applicative verb"@en ;
                 
                 rdfs:subClassOf :DeverbalVerb ;
                 
                 :example "German: \"steigen\"(V) 'rise' --> \"besteigen\"(V) 'climb'."@de ;
                 
                 rdfs:comment "A verb which is derived from another intransitive verb stem resulting in a transitive verb."@en ;
                 
                 rdfs:seeAlso """Christian Lehmann, under \"applicative verb\" at http://linguistik.uni-erfurt.de:8080/lido/Lido :
An applicative verb is a derived transitive verb whose direct object has been promoted to this function from a more peripheral syntactic function that it has with the base verb.

The base may be transitive, in which case its direct object is demoted upon the derivation of the applicative verb."""@en .



###  http://mmoon.org/mmoon/AtomicMorpheme

:AtomicMorpheme rdf:type owl:Class ;
                
                rdfs:label "Atomic morpheme"@en ;
                
                rdfs:subClassOf :Morpheme ;
                
                rdfs:comment """A morpheme is atomic if the morph by which it is realized encodes exactly one meaning. Hence, an atomic morpheme has one mmon:Meaning. 

An exception is made for person and number morphemes, e.g. the third person singular \"-s\" suffix in English corresponds to the atomic morpheme \"1SG\"."""@en ;
                
                :example "The English \"-s\" plural morpheme."@en .



###  http://mmoon.org/mmoon/AugmentativeNoun

:AugmentativeNoun rdf:type owl:Class ;
                  
                  rdfs:label "Augmentative noun"@en ;
                  
                  rdfs:subClassOf :DenominalNoun ;
                  
                  rdfs:comment "A noun which is derived from another noun stem that denotes big or large size. Possible connotations include strong, imposing, ugly."@en ;
                  
                  rdfs:seeAlso """Christian Lehmann, under \"augmentation\" at http://linguistik.uni-erfurt.de:8080/lido/Lido :
Augmentation is the derivational modification of a noun by the concept „big, large“. Possible connotations include „strong, imposing, ugly“.
A noun is augmentative 1 iff it is derived by augmentation."""@en ,
                               gold:AugmentativeSize ,
                               <http://purl.org/olia/olia.owl#Augmentative> .



###  http://mmoon.org/mmoon/CausativeVerb

:CausativeVerb rdf:type owl:Class ;
               
               rdfs:label "Causative verb"@en ;
               
               rdfs:subClassOf :DeverbalVerb ;
               
               rdfs:comment "A verb which is derived from another verb stem denoting  the causal role of a referent in relation to an event or state expressed by the deriving verb stem."@en ;
               
               rdfs:seeAlso """Christian Lehmann, under \"causative verb\" at http://linguistik.uni-erfurt.de:8080/lido/Lido : 
A causative verb is an n-place verb (with n > 1) which is derived from an n-1-place verb in such a way that the additional semantic slot is mapped onto the subject slot and is occupied by a superordinate agent which causes the situation designated by the base.

An underived verb cannot be causative by this definition. However, the paradigmatic lexical relation of Engl. «kill» to «die» may be called ‚semantically causative’."""@en ;
               
               :example """Eng.: \"fall\"(V) --> \"fell\"(V).
[Christian Lehmann, under \"causative verb\" at http://linguistik.uni-erfurt.de:8080/lido/Lido]"""@en .



###  http://mmoon.org/mmoon/Circumfix

:Circumfix rdf:type owl:Class ;
           
           rdfs:label "Circumfix"@en ;
           
           owl:equivalentClass gold:Circumfix ;
           
           rdfs:subClassOf :Affix ;
           
           rdfs:comment "A circumfix is an affix which consits of a prefix and a suffix. [Christian Lehmann, under \"circumfix\" at http://linguistik.uni-erfurt.de:8080/lido/Lido ]"@en .



###  http://mmoon.org/mmoon/CollectivePersonNoun

:CollectivePersonNoun rdf:type owl:Class ;
                      
                      rdfs:label "Collective person noun"@en ;
                      
                      rdfs:subClassOf :DenominalNoun ;
                      
                      :example "German: \"Lehrer\"(N) 'teacher' --> \"Lehrerschaft\"(N) 'body of teachers'."@de ;
                      
                      rdfs:comment "A noun which is derived from another noun stem that denotes group of persons."@en .



###  http://mmoon.org/mmoon/ComplexMorpheme

:ComplexMorpheme rdf:type owl:Class ;
                 
                 rdfs:label "Complex morpheme"@en ;
                 
                 rdfs:subClassOf :Morpheme ;
                 
                 rdfs:comment "A  morpheme is complex if it corresponds to more than one morph, and therefore consists of fusional and/or atomic and/or empty morphemes."@en ;
                 
                 :example "The English noun stem \"driver\" consists of the verbal stem \"drive\" and the derivational suffix \"-er\". The corresponding complex morpheme is \"drive.PRS-AG.NMLZ\", which consists of the two fusional morphemes \"drive.PRS\" and \"AG.NMLZ\"."@en ;
                 
                 :usageNote """The declaration of such a morpheme is somewhat contrary to the definition of morpheme as \"smallest meaning-bearing units of a language\". Since each mmoon:Morph resource should be able to correspond to some morpheme the construct of a complex morpheme is established. This is often the case for derived stems.
 In the URI of the complex morpheme the morphemes of which it consists are separated by a hyphen."""@en .



###  http://mmoon.org/mmoon/CompoundWord

:CompoundWord rdf:type owl:Class ;
              
              rdfs:label "Compound Word"@en ;
              
              owl:equivalentClass gold:Compound ;
              
              rdfs:subClassOf :Lexeme ,
                              [ rdf:type owl:Restriction ;
                                owl:onProperty :isComposedOf ;
                                owl:onClass [ rdf:type owl:Class ;
                                              owl:unionOf ( :GrammaticalWord
                                                            :Lexeme
                                                          )
                                            ] ;
                                owl:qualifiedCardinality "2"^^xsd:nonNegativeInteger
                              ] ,
                              [ rdf:type owl:Restriction ;
                                owl:onProperty :compoundingRelation ;
                                owl:someValuesFrom :Compounding
                              ] ;
              
              rdfs:comment """A compound is a stem formed by composition. [Christian Lehmann, under \"compound\" at http://linguistik.uni-erfurt.de:8080/lido/Lido]

Is a kind of lexeme which is formed by the combination of two stems."""@en ;
              
              :example "Engl. \"playground\"."@en ;
              
              :usageNote "The compound word is specified for the two stems of which it is composed by using the property :consistsOfMorph, thus explicating the morphs which are involved in the word-formation of the compound word."@en .



###  http://mmoon.org/mmoon/Compounding

:Compounding rdf:type owl:Class ;
             
             rdfs:label "Compounding"@en ;
             
             rdfs:subClassOf :WordFormation ;
             
             rdfs:seeAlso """Christian Lehmann, under \"compounding\" at http://linguistik.uni-erfurt.de:8080/lido/Lido :
Compounding [compositio thematum] is the formation of a stem by combination of two stems. Both stems may already be complex."""@en ;
             
             :usageNote "Compounds, in English and some other languages, can be written as one word or two separate words, and they can be hyphenated as well. [http://www.glottopedia.org/index.php/Compound]"@en ;
             
             rdfs:comment "Is the process of lexeme-formation by combining two stems."@en .



###  http://mmoon.org/mmoon/Conjugation

:Conjugation rdf:type owl:Class ;
             
             rdfs:label "Conjugation"@en ;
             
             rdfs:subClassOf :VerbalInflection ;
             
             rdfs:comment "Is the inflection of a verb. Conjugation categories commonly include person, number, gender, aspect, tense, mood, voice and non-finite subcategories. [Christian Lehmann, under \"conjugation\" at http://linguistik.uni-erfurt.de:8080/lido/Lido ]"@en .



###  http://mmoon.org/mmoon/Conversion

:Conversion rdf:type owl:Class ;
            
            rdfs:label "Conversion"@en ;
            
            rdfs:subClassOf :Derivation ;
            
            :usageNote "All other derivations which include an affix marking the wordclass-change but also do not entail further derivational meaning belong into the according mmoon:Derived[Wordclass] subclasses."@en ;
            
            rdfs:seeAlso """Christian Lehmann, under \"conversion\" at http://linguistik.uni-erfurt.de:8080/lido/Lido :
Conversion [recategorizatio] is the implicit change of the word class of a stem.
Conversion [recategorizatio] is not a kind of derivation 1 if the latter is conceived as involving a morphological process. At the level of formal representation, however, conversion [recategorizatio] may be conceived as dependency of a stem on a zero affix."""@en ;
            
            rdfs:comment "Conversion, also called zero-derivation, is the formation of a lexeme from another part of speech which entails no further derivational meaning except that which is entailed in the wordclass-change."@en ;
            
            rdfs:seeAlso <http://www.glottopedia.org/index.php/Conversion> .



###  http://mmoon.org/mmoon/DeadjectivalAdjective

:DeadjectivalAdjective rdf:type owl:Class ;
                       
                       rdfs:label "Deadjectival adjective"@en ;
                       
                       rdfs:subClassOf :DerivedAdjective ;
                       
                       rdfs:comment "Is an adjective lexeme which derived from another adjective stem."@en .



###  http://mmoon.org/mmoon/DeadjectivalAdverb

:DeadjectivalAdverb rdf:type owl:Class ;
                    
                    rdfs:label "DeadjectivalAdverb"@en ;
                    
                    rdfs:subClassOf :DerivedAdverb ;
                    
                    :usageNote "Add instance here, if the language of the given morpheme inventory exhibits affixal marking for word-class change but adds NO further derivational meaning(s). For all derived lexemes that consist of a derivational affix denoting some additional meaning, the respective subclass must be instantiated or newly created."@en ;
                    
                    rdfs:comment "Is an adverb lexeme which derived from an adjective stem."@en .



###  http://mmoon.org/mmoon/DeadjectivalNoun

:DeadjectivalNoun rdf:type owl:Class ;
                  
                  rdfs:label "Deadjectival noun"@en ;
                  
                  rdfs:subClassOf :DerivedNoun ;
                  
                  :usageNote "Add instance here, if the language of the given morpheme inventory exhibits affixal marking for word-class change but adds NO further derivational meaning(s). For all derived lexemes that consist of a derivational affix denoting some additional meaning, the respective subclass must be instantiated or newly created."@en ;
                  
                  rdfs:comment "Is a noun lexeme which derived from an adjective stem."@en .



###  http://mmoon.org/mmoon/DeadjectivalVerb

:DeadjectivalVerb rdf:type owl:Class ;
                  
                  rdfs:label "Deadjectival verb"@en ;
                  
                  rdfs:subClassOf :DerivedVerb ;
                  
                  :usageNote "Add instance here, if the language of the given morpheme inventory exhibits affixal marking for word-class change but adds NO further derivational meaning(s). For all derived lexemes that consist of a derivational affix denoting some additional meaning, the respective subclass must be instantiated or newly created."@en ;
                  
                  rdfs:comment "Is a verb lexeme which derived from an adjective stem."@en .



###  http://mmoon.org/mmoon/DeadverbalAdverb

:DeadverbalAdverb rdf:type owl:Class ;
                  
                  rdfs:label "Deadverbal adverb"@en ;
                  
                  rdfs:subClassOf :DerivedAdverb ;
                  
                  rdfs:comment "Is an adverb lexeme which derived from another adverb stem."@en .



###  http://mmoon.org/mmoon/Declension

:Declension rdf:type owl:Class ;
            
            rdfs:label "Declension"@en ;
            
            rdfs:subClassOf :NominalInflection ;
            
            rdfs:comment "Is the inflection of a noun. Relevant categories commonly include gender, number, case, possessive and definiteness. [Christian Lehmann, under \"declension\" at http://linguistik.uni-erfurt.de:8080/lido/Lido ]"@en .



###  http://mmoon.org/mmoon/Degree

:Degree rdf:type owl:Class ;
        
        rdfs:label "Degree"@en ;
        
        rdfs:subClassOf :AdjectivalInflection ;
        
        rdfs:comment "Attributively (but also predicatively) used adjectives inflect for the category degree of comparison. In agreement with the noun it modifies it can also be marked for nominal inflectional categories such as gender, case and number."@en .



###  http://mmoon.org/mmoon/DenominalAdjective

:DenominalAdjective rdf:type owl:Class ;
                    
                    rdfs:label "Denominal adjective"@en ;
                    
                    rdfs:subClassOf :DerivedAdjective ;
                    
                    :usageNote "Add instance here, if the language of the given morpheme inventory exhibits affixal marking for word-class change but adds NO further derivational meaning(s). For all derived lexemes that consist of a derivational affix denoting some additional meaning, the respective subclass must be instantiated or newly created."@en ;
                    
                    rdfs:comment "Is an adjective lexeme which derived from noun stem."@en .



###  http://mmoon.org/mmoon/DenominalAdverb

:DenominalAdverb rdf:type owl:Class ;
                 
                 rdfs:label "Denominal adverb"@en ;
                 
                 rdfs:subClassOf :DerivedAdverb ;
                 
                 :usageNote "Add instance here, if the language of the given morpheme inventory exhibits affixal marking for word-class change but adds NO further derivational meaning(s). For all derived lexemes that consist of a derivational affix denoting some additional meaning, the respective subclass must be instantiated or newly created."@en ;
                 
                 rdfs:comment "Is an adverb lexeme which derived from a noun stem."@en .



###  http://mmoon.org/mmoon/DenominalNoun

:DenominalNoun rdf:type owl:Class ;
               
               rdfs:label "Denominal noun"@en ;
               
               rdfs:subClassOf :DerivedNoun ;
               
               rdfs:comment "Is a noun lexeme which derived from another noun stem."@en .



###  http://mmoon.org/mmoon/DenominalVerb

:DenominalVerb rdf:type owl:Class ;
               
               rdfs:label "Denominal verb"@en ;
               
               rdfs:subClassOf :DerivedVerb ;
               
               :usageNote "Add instance here, if the language of the given morpheme inventory exhibits affixal marking for word-class change but adds NO further derivational meaning(s). For all derived lexemes that consist of a derivational affix denoting some additional meaning, the respective subclass must be instantiated or newly created."@en ;
               
               rdfs:comment "Is a verb lexeme which derived from a noun stem."@en .



###  http://mmoon.org/mmoon/Derivation

:Derivation rdf:type owl:Class ;
            
            rdfs:label "Derivation"@en ;
            
            rdfs:subClassOf :WordFormation ;
            
            rdfs:comment "Is the process of lexeme-formation which is morphologically conditioned and involves the modification of a stem."@en .



###  http://mmoon.org/mmoon/DerivedAdjective

:DerivedAdjective rdf:type owl:Class ;
                  
                  rdfs:label "Derived adjective"@en ;
                  
                  rdfs:subClassOf :Derivation ;
                  
                  rdfs:comment "Is an adjective lexeme which derived from another stem."@en .



###  http://mmoon.org/mmoon/DerivedAdverb

:DerivedAdverb rdf:type owl:Class ;
               
               rdfs:label "Derived adverb"@en ;
               
               rdfs:subClassOf :Derivation ;
               
               rdfs:comment "Is an adverb lexeme which derived from another stem."@en .



###  http://mmoon.org/mmoon/DerivedNoun

:DerivedNoun rdf:type owl:Class ;
             
             rdfs:label "Derived noun"@en ;
             
             rdfs:subClassOf :Derivation ;
             
             rdfs:comment "Is a noun lexeme which derived from another stem."@en .



###  http://mmoon.org/mmoon/DerivedVerb

:DerivedVerb rdf:type owl:Class ;
             
             rdfs:label "Derived verb"@en ;
             
             rdfs:subClassOf :Derivation ;
             
             rdfs:comment "Is a verb lexeme which derived from another stem."@en .



###  http://mmoon.org/mmoon/DerivedWord

:DerivedWord rdf:type owl:Class ;
             
             rdfs:label "Derived word"@en ;
             
             rdfs:subClassOf :Lexeme ,
                             [ rdf:type owl:Restriction ;
                               owl:onProperty :derivationalRelation ;
                               owl:someValuesFrom :Derivation
                             ] ,
                             [ rdf:type owl:Restriction ;
                               owl:onProperty :isDerivedFrom ;
                               owl:onClass [ rdf:type owl:Class ;
                                             owl:unionOf ( :GrammaticalWord
                                                           :Lexeme
                                                         )
                                           ] ;
                               owl:qualifiedCardinality "1"^^xsd:nonNegativeInteger
                             ] ;
             
             :example "\"replay\" is a derived word from the lexeme \"play\"."@en ;
             
             rdfs:comment """A derivate is a stem generated by derivation [derivatio]. [Christian Lehmann, under \"derivate\" at http://linguistik.uni-erfurt.de:8080/lido/Lido]

Is a kind of lexeme which is formed by the morphological modification of another lexical stem."""@en ;
             
             :usageNote "The derived word is specified for the stem from which it is derived as well as for the affix that is involved in the derivation by using the property :consistsOfMorph, thus explicating the morphs which are involved in the word-formation of the derived word."@en .



###  http://mmoon.org/mmoon/DesiderativeVerb

:DesiderativeVerb rdf:type owl:Class ;
                  
                  rdfs:label "Desiderative verb"@en ;
                  
                  rdfs:subClassOf :DeverbalVerb ;
                  
                  rdfs:comment "A verb which is derived from another verb stem denoting to want the meaning of the deriving verb stem."@en ;
                  
                  :example "Sanskrit: \"‚s:r.no-ti\" (V) 'hears' --> \"‚su-’sr¡u-.sa-ti\"(V) (RED-hear-DES-3.SG) 'wants to hear'."@sa .



###  http://mmoon.org/mmoon/DeverbalAdjective

:DeverbalAdjective rdf:type owl:Class ;
                   
                   rdfs:label "Deverbal Adjective"@en ;
                   
                   rdfs:subClassOf :DerivedAdjective ;
                   
                   :usageNote "Add instance here, if the language of the given morpheme inventory exhibits affixal marking for word-class change but adds NO further derivational meaning(s). For all derived lexemes that consist of a derivational affix denoting some additional meaning, the respective subclass must be instantiated or newly created."@en ;
                   
                   rdfs:comment "Is an adjective lexeme which derived from a verb stem."@en .



###  http://mmoon.org/mmoon/DeverbalAdverb

:DeverbalAdverb rdf:type owl:Class ;
                
                rdfs:label "Deverbal adverb"@en ;
                
                rdfs:subClassOf :DerivedAdverb ;
                
                :usageNote "Add instance here, if the language of the given morpheme inventory exhibits affixal marking for word-class change but adds NO further derivational meaning(s). For all derived lexemes that consist of a derivational affix denoting some additional meaning, the respective subclass must be instantiated or newly created."@en ;
                
                rdfs:comment "Is an adverb lexeme which derived from a verb stem."@en .



###  http://mmoon.org/mmoon/DeverbalNoun

:DeverbalNoun rdf:type owl:Class ;
              
              rdfs:label "Deverbal noun"@en ;
              
              rdfs:subClassOf :DerivedNoun ;
              
              :usageNote "Add instance here, if the language of the given morpheme inventory exhibits affixal marking for word-class change but adds NO further derivational meaning(s). For all derived lexemes that consist of a derivational affix denoting some additional meaning, the respective subclass must be instantiated or newly created."@en ;
              
              rdfs:comment "Is a noun lexeme which derived from a verb stem."@en .



###  http://mmoon.org/mmoon/DeverbalVerb

:DeverbalVerb rdf:type owl:Class ;
              
              rdfs:label "Deverbal verb"@en ;
              
              rdfs:subClassOf :DerivedVerb ;
              
              rdfs:comment "Is a verb lexeme which derived from another verb stem."@en .



###  http://mmoon.org/mmoon/DiminutiveAdjective

:DiminutiveAdjective rdf:type owl:Class ;
                     
                     rdfs:label "Diminutive adjective"@en ;
                     
                     rdfs:subClassOf :DeadjectivalAdjective ;
                     
                     rdfs:seeAlso "http://purl.org/linguistics/gold/DiminuativeSize" ;
                     
                     rdfs:comment "An adjective which is derived from another adjective stem that denotes a smaller intensity than the deriving adjective stem."@en ;
                     
                     :example "Eng. \"small\"(ADJ) --> \"smallish\"(ADJ)"@en .



###  http://mmoon.org/mmoon/DiminutiveNoun

:DiminutiveNoun rdf:type owl:Class ;
                
                rdfs:label "Diminutive noun"@en ;
                
                rdfs:subClassOf :DenominalNoun ;
                
                :example "German \"Kind\"(N) --> \"Kindchen\"(N)"@de ;
                
                rdfs:comment "A noun which is derived from another noun stem that denotes endearment, small size or small intensity."@en ;
                
                :example "Eng. \"duck\"(N) --> \"duckling\"(N)"@en ;
                
                rdfs:seeAlso gold:DiminuativeSize ,
                             <http://purl.org/olia/olia.owl#DiminutiveNoun> .



###  http://mmoon.org/mmoon/EmptyMorph

:EmptyMorph rdf:type owl:Class ;
            
            rdfs:label "Empty morph"@en ;
            
            rdfs:subClassOf :Affix ,
                            [ rdf:type owl:Restriction ;
                              owl:onProperty :correspondsToMorpheme ;
                              owl:allValuesFrom :EmptyMorpheme
                            ] ;
            
            rdfs:comment "A morph that has no meaning but that must be posited for the sake of descriptive elegance. [Haspelmath and Sims: Understanding morphology. 2002:327]"@en .



###  http://mmoon.org/mmoon/EmptyMorpheme

:EmptyMorpheme rdf:type owl:Class ;
               
               rdfs:label "Empty morpheme"@en ;
               
               rdfs:subClassOf :Morpheme ;
               
               :usageNote "An empty morpheme is realized by an empty morph. Often an empty morph is realized for the sake of euphony."@en ;
               
               rdfs:comment "An empty morpheme serves as means to state that a morph (except for the zero morph) corresponds to no meaning."@en .



###  http://mmoon.org/mmoon/FactitiveVerb

:FactitiveVerb rdf:type owl:Class ;
               
               rdfs:label "Factitive verb"@en ;
               
               rdfs:subClassOf :DeadjectivalVerb ;
               
               :example """German: \"tot\"(Adj) 'dead' --> \"töten\"(V) 'to kill'.
 [Christian Lehmann, under \"factitive verb\" at http://linguistik.uni-erfurt.de:8080/lido/Lido]"""@de ;
               
               rdfs:comment "A verb which is derived from an adjective stem denoting causation."@en ;
               
               rdfs:seeAlso """Christian Lehmann, under \"factitive verb\" at http://linguistik.uni-erfurt.de:8080/lido/Lido :
A factitive verb is a causative verb based on an adjective (or a stative intransitive verb).

Delimitation and History:
While there may be a subordinate agent in a causative construction, there may be none in a factitive one. This has sometimes been a reason for not subsuming factitive under causative."""@en ;
               
               :example """Engl.:\"black\"(Adj) --> \"blacken\"(Vtr.).
 [Christian Lehmann, under \"factitive verb\" at http://linguistik.uni-erfurt.de:8080/lido/Lido]"""@en .



###  http://mmoon.org/mmoon/FemaleNoun

:FemaleNoun rdf:type owl:Class ;
            
            rdfs:label "Female noun"@en ;
            
            rdfs:subClassOf :DenominalNoun ;
            
            :example "German: \"Fahrer\"(N) 'male driver' --> \"Fahrerin\"(N) 'female driver'."@de ;
            
            rdfs:comment "A noun which is derived from another noun stem and that denotes a female person."@en .



###  http://mmoon.org/mmoon/FusionalMorpheme

:FusionalMorpheme rdf:type owl:Class ;
                  
                  rdfs:label "Fusional morpheme"@en ;
                  
                  rdfs:subClassOf :Morpheme ;
                  
                  rdfs:comment """A morpheme is fusional if it entails more than one meaning and if these meanings are expressed in one un-analyzable morph. Hence, a fusional morpheme has at least two mmon:Meaning(s). Each meaning is separated by a period in the URI of a fusional morpheme instance.
This often the case for inherent meanings such as number for nouns or tense for verbs."""@en ;
                  
                  :example "The English stem \"go\" of the verb \"to go\"  is a morph encoding the meaning of the root \"go\" and inherently also present tense. It corresponds to the fusional morpheme \"go.PRS\""@en .



###  http://mmoon.org/mmoon/GrammaticalWord

:GrammaticalWord rdf:type owl:Class ;
                 
                 rdfs:label "Grammatical word"@en ;
                 
                 rdfs:subClassOf :Word ;
                 
                 rdfs:comment "A grammatical word is a word which is a grammatical formative. [Christian Lehmann, under \"grammatical word\" at http://linguistik.uni-erfurt.de:8080/lido/Lido]"@en ;
                 
                 :example "Engl. «be», «of».  [Christian Lehmann, under \"grammatical word\" at http://linguistik.uni-erfurt.de:8080/lido/Lido]"@en .



###  http://mmoon.org/mmoon/Infix

:Infix rdf:type owl:Class ;
       
       rdfs:label "Infix"@en ;
       
       owl:equivalentClass gold:Infix ;
       
       rdfs:subClassOf :Affix ;
       
       rdfs:comment "An infix is an affix that is added within an otherwise unanalysable root and disrupts this. [Christian Lehmann, under \"infix\" at http://linguistik.uni-erfurt.de:8080/lido/Lido ]"@en .



###  http://mmoon.org/mmoon/Inflection

:Inflection rdf:type owl:Class ;
            
            rdfs:label "Inflection"@en ;
            
            rdfs:subClassOf :MorphologicalRelationship ;
            
            rdfs:seeAlso """Christian Lehmann, under \"inflection\" at http://linguistik.uni-erfurt.de:8080/lido/Lido] :
Inflection [flexio] is the syntactically relevant part of morphology. It generates word forms (inflectional forms) of word stems.
In contrast to derivation, inflection  never results in a change of word class and produces a predictable, regular change of meaning (for regular word-forms only).
Its expression is typically located farther from the root than that of derivation."""@en ;
            
            :usageNote "In the subclasses of \"Inflection\" the semantic or grammatic categories are not extensively specified. They only serve to declare what kind of morphological relationship(s) is/are expressed on a word-form."@en ;
            
            rdfs:comment "Is the process of generating word-forms of lexical stems. This class can be extended to describe the inflectional classes of the lexemes of a language."@en .



###  http://mmoon.org/mmoon/InstrumentNoun

:InstrumentNoun rdf:type owl:Class ;
                
                rdfs:label "Instrument noun"@en ;
                
                rdfs:subClassOf :DeverbalNoun ;
                
                :example "German: \"lenken\"(V) 'to steer'--> \"Lenker\"(N) 'handle-bar, steering wheel'. [Christian Lehmann, under \"instrument noun\" at http://linguistik.uni-erfurt.de:8080/lido/Lido]"@de ;
                
                rdfs:comment "A noun which is derived from a verb stem denoting that some thing/instrument is used to carry out the meaning of the verb stem."@en ;
                
                rdfs:seeAlso """Christian Lehmann, under \"instrument noun\" at http://linguistik.uni-erfurt.de:8080/lido/Lido :
An instrument noun is an oriented deverbal noun that designates something that functions as an instrument in the situation designated by the base verb. [Christian Lehmann, under \"instrument noun\" at http://linguistik.uni-erfurt.de:8080/lido/Lido]"""@en .



###  http://mmoon.org/mmoon/Introflection

:Introflection rdf:type owl:Class ;
               
               rdfs:label "Introflection"@en ;
               
               rdfs:subClassOf :Inflection ,
                               :WordFormation ;
               
               rdfs:comment "Nonconcatenative morphology, also called discontinuous morphology and introflection, is a form of word-formation [and inflection] in which the root is modified and does not involve stringing morphemes together. [Haspelmath and Sims: Understanding morphology. 2002, Sections 3.1.2 - 3.1.4]"@en .



###  http://mmoon.org/mmoon/IrregularConjugation

:IrregularConjugation rdf:type owl:Class ;
                      
                      rdfs:label "Irregular conjugation"@en ;
                      
                      rdfs:subClassOf :Conjugation ;
                      
                      rdfs:comment "Conjugation that deviates from the regular inflectional pattern."@en .



###  http://mmoon.org/mmoon/IrregularDegree

:IrregularDegree rdf:type owl:Class ;
                 
                 rdfs:label "Irregular degree"@en ;
                 
                 rdfs:subClassOf :Degree ;
                 
                 rdfs:comment "Formation of degree of comparison that deviates from the regular inflectional pattern."@en .



###  http://mmoon.org/mmoon/Lexeme

:Lexeme rdf:type owl:Class ;
        
        rdfs:label "Lexeme"@en ;
        
        owl:equivalentClass gold:LexicalItem ;
        
        rdfs:subClassOf :Word ;
        
        rdfs:comment "A lexeme is a word as it appears as an entry in a dictionary. It has a holistic abstract sense representing the core meaning shared by a set of closely-related word-forms. A lexeme can only be a word that inflects."@en ;
        
        rdfs:seeAlso """Christian Lehmann, under \"lexeme\" at http://linguistik.uni-erfurt.de:8080/lido/Lido :
A lexeme [lexema] is a word in its capacity as a unit of the lexicon. In a text, it appears in form of diverse word forms."""@en .



###  http://mmoon.org/mmoon/MaterialAdjective

:MaterialAdjective rdf:type owl:Class ;
                   
                   rdfs:label "Material adjective"@en ;
                   
                   rdfs:subClassOf :DenominalAdjective ;
                   
                   :example "German: Holz 'wood' --> hölzern 'wooden'."@de ;
                   
                   rdfs:comment "An adjective which is derived from a noun stem denoting some kind of material and means 'being made of this material'."@en .



###  http://mmoon.org/mmoon/Meaning

:Meaning rdf:type owl:Class ;
         
         rdfs:label "Meaning"@en ;
         
         rdfs:comment "This class comprises a wide range of meanings a linguistic sign can be associated with, e.g. linguistic categories, morphosyntactic features, lexical senses, derivational meanings."@en .



###  http://mmoon.org/mmoon/Morph

:Morph rdf:type owl:Class ;
       
       rdfs:label "Morph"@en ;
       
       rdfs:subClassOf [ rdf:type owl:Restriction ;
                         owl:onProperty :hasRepresentation ;
                         owl:someValuesFrom :Representation
                       ] ;
       
       rdfs:comment "A morph is a concrete realization of a single morpheme which usually results from segmentation."@en ;
       
       :usageNote "A morph resource describes only the perceptible side of a morpheme, i.e. the significans. As such it is not directly associated with a meaning but with a corresponding morpheme resource."@en .



###  http://mmoon.org/mmoon/Morpheme

:Morpheme rdf:type owl:Class ;
          
          rdfs:label "Morpheme"@en ;
          
          rdfs:subClassOf [ rdf:type owl:Restriction ;
                            owl:onProperty :hasMeaning ;
                            owl:onClass :Meaning ;
                            owl:minQualifiedCardinality "1"^^xsd:nonNegativeInteger
                          ] ;
          
          :usageNote """A morpheme resource describes only the conceptual side, i.e. the significatum, which is realized by one or more morphs in a certain language. Thus, the meaning(s) it conveys must be always stated via the mmoon:hasMeaning property.

For convenience the morpheme instances are rendered by the same notatinal means as the morphemic glosses, i.e. the plural morpheme is rendered in short as \"PL\"."""@en ;
          
          rdfs:comment """The morpheme class usually contains the smallest meaning-bearing units of a language. These comprise all semantically or grammatically distinct parts which are identifiable by segmentation of  the morphs of which a word or a word-form consists.

Depending on the kind of correspondence betweene a morpheme its morph realization, four kinds of morphemes are established: 1) atomic morphemes, 2) fusional morphemes, 3) Empty morphemes and 4) complex morphemes."""@en .



###  http://mmoon.org/mmoon/MorphemeInventory

:MorphemeInventory rdf:type owl:Class ;
                   
                   rdfs:label "Morpheme inventory"@en ;
                   
                   rdfs:comment "The morpheme inventory is the object that contains morphemic entries. It is specified for the natural language it describes."@en .



###  http://mmoon.org/mmoon/MorphemicGloss

:MorphemicGloss rdf:type owl:Class ;
                
                rdfs:label "Morphemic gloss"@en ;
                
                rdfs:comment "The gloss is the abstract identity of a morpheme. It serves as a metalinguistic representation of morphological meanings. Most of the glosses used for grammatical concepts are taken from the Leipzig Glossing Rules  (https://www.eva.mpg.de/lingua/pdf/LGR08.02.05.pdf) or from Lehmann 2004 (http://christianlehmann.eu/publ/img.pdf). Lexical senses are usually glossed in English by using the orthographic representation of the lexical element (such as stems and roots) but can be also given in the language of the MMoOn language inventory."@en .



###  http://mmoon.org/mmoon/MorphologicalRelationship

:MorphologicalRelationship rdf:type owl:Class ;
                           
                           rdfs:label "Morphological Relationship"@en ;
                           
                           rdfs:comment "Is the relationship between word-forms of a lexeme (inflection) or the relationship between lexemes of a word family (derivation and compounding). [Haspelmath and Sims: Understanding morphology. 2002:18]"@en .



###  http://mmoon.org/mmoon/NoDegree

:NoDegree rdf:type owl:Class ;
          
          rdfs:label "No degree"@en ;
          
          rdfs:subClassOf :AdjectivalInflection ;
          
          rdfs:comment "Some adjectives do not inflect for the category degree of comparison, e.g. \"dead\", \"absolute\", \"pregnant\". In agreement with the noun it modifies it can still be marked for nominal inflectional categories such as gender, case and number."@en .



###  http://mmoon.org/mmoon/NoInflection

:NoInflection rdf:type owl:Class ;
              
              rdfs:label "No inflection"@en ;
              
              rdfs:subClassOf :Inflection ;
              
              rdfs:comment "This class marks words which do not inflect. This holds for most grammatical words but also for some lexemes (e.g. the invariable adjective \"super\" in German)."@en .



###  http://mmoon.org/mmoon/NoWordFormation

:NoWordFormation rdf:type owl:Class ;
                 
                 rdfs:label "No word-formation"@en ;
                 
                 rdfs:subClassOf :WordFormation ;
                 
                 rdfs:comment "Simple lexemes that cannot be further segmented into derivational or compositional components exhibit no kind of word-formation. Rather, they serve as the derivational or compositional basis for derived words and compound words."@en .



###  http://mmoon.org/mmoon/NominalAdverb

:NominalAdverb rdf:type owl:Class ;
               
               rdfs:label "Nominal adverb"@en ;
               
               rdfs:subClassOf :Conversion ;
               
               rdfs:comment "A nominal adverb is an adverb which is fomed by conversion from a noun and which entails no further derivational meaning except the entailed wordclass-change."@en ;
               
               :example "Engl.: \"backstage\"(N) --> \"backstage\"(Adv)."@en .



###  http://mmoon.org/mmoon/NominalCompound

:NominalCompound rdf:type owl:Class ;
                 
                 rdfs:label "Nominal compound"@en ;
                 
                 rdfs:subClassOf :Compounding ;
                 
                 rdfs:comment "A nominal compound is a noun formed by composition of a nominal stem and another stem."@en ;
                 
                 :example "Engl.: \"blackboard\"(N) = \"black\"(Adj) + \"board\"(N)."@en .



###  http://mmoon.org/mmoon/NominalInflection

:NominalInflection rdf:type owl:Class ;
                   
                   rdfs:label "Nominal inflection"@en ;
                   
                   rdfs:subClassOf :Inflection ;
                   
                   rdfs:comment "Is the process of generating word-forms of nominal stems."@en .



###  http://mmoon.org/mmoon/NominalVerb

:NominalVerb rdf:type owl:Class ;
             
             rdfs:label "Nominal verb"@en ;
             
             rdfs:subClassOf :Conversion ;
             
             rdfs:comment "A nominal verb is a verb which is fomed by conversion from a noun and which entails no further derivational meaning except the entailed wordclass-change."@en ;
             
             :example "Engl.: \"the steam\"(N) --> \"to steam\"(V)."@en .



###  http://mmoon.org/mmoon/NounAdjective

:NounAdjective rdf:type owl:Class ;
               
               rdfs:label "Noun adjective"@en ;
               
               rdfs:subClassOf :Conversion ;
               
               rdfs:comment "A noun adjective is an adjective which is fomed by conversion from a noun and which entails no further derivational meaning except the entailed wordclass-change."@en ;
               
               :example "Engl.: \"Swiss\"(NPr) --> \"Swiss\"(Adj)."@en .



###  http://mmoon.org/mmoon/PredicativeAdj

:PredicativeAdj rdf:type owl:Class ;
                
                rdfs:label "Predicative adjective"@en ;
                
                rdfs:subClassOf :AdjectivalInflection ;
                
                rdfs:comment "Predicatively used adjectives (in sentences such as \"Peter is small.\") charactarize the noun when occuring with copula verbs like \"be\" and do not inflect for nominal agreement. Relational adjectives (i.e. gradable adjectives) do still inflect for degree."@en .



###  http://mmoon.org/mmoon/Prefix

:Prefix rdf:type owl:Class ;
        
        rdfs:label "Prefix"@en ;
        
        owl:equivalentClass gold:Prefix ;
        
        rdfs:subClassOf :Affix ;
        
        rdfs:comment "A prefix is an affix that precedes its stem or root. [Christian Lehmann, under \"prefix\" at http://linguistik.uni-erfurt.de:8080/lido/Lido ]"@en .



###  http://mmoon.org/mmoon/RegularConjugation

:RegularConjugation rdf:type owl:Class ;
                    
                    rdfs:label "Regular conjugation"@en ;
                    
                    rdfs:subClassOf :Conjugation ;
                    
                    rdfs:comment "Conjugation that exhibits a regular inflectional pattern."@en .



###  http://mmoon.org/mmoon/RegularDegree

:RegularDegree rdf:type owl:Class ;
               
               rdfs:label "Regular degree"@en ;
               
               rdfs:subClassOf :Degree ;
               
               rdfs:comment "Formation of degree of comparison that exhibits a regular inflectional pattern."@en .



###  http://mmoon.org/mmoon/Representation

:Representation rdf:type owl:Class ;
                
                rdfs:label "Representation"@en ;
                
                rdfs:subClassOf [ rdf:type owl:Class ;
                                  owl:unionOf ( [ rdf:type owl:Restriction ;
                                                  owl:onProperty :orthographicRepresentation ;
                                                  owl:minQualifiedCardinality "1"^^xsd:nonNegativeInteger ;
                                                  owl:onDataRange xsd:string
                                                ]
                                                [ rdf:type owl:Restriction ;
                                                  owl:onProperty :phoneticRepresentation ;
                                                  owl:minQualifiedCardinality "1"^^xsd:nonNegativeInteger ;
                                                  owl:onDataRange xsd:string
                                                ]
                                              )
                                ] ;
                
                rdfs:comment "A linguistic representation of a word or morph.."@en .



###  http://mmoon.org/mmoon/Root

:Root rdf:type owl:Class ;
      
      rdfs:label "Root"@en ;
      
      owl:equivalentClass gold:Root ;
      
      rdfs:subClassOf :Morph ;
      
      rdfs:comment "A morph that constitutes the semantic nucleus of a stem. It cannot be further segmented and is often not specified for a part of speech. There are lexical roots, like Engl. «get», and grammatical roots, like Engl. «wh-». [Christian Lehmann, under \"root\" at http://linguistik.uni-erfurt.de:8080/lido/Lido ]"@en .



###  http://mmoon.org/mmoon/Simulfix

:Simulfix rdf:type owl:Class ;
          
          rdfs:label "Simulfix"@en ;
          
          rdfs:subClassOf :Affix ;
          
          rdfs:isDefinedBy "http://www-01.sil.org/linguistics/GlossaryOflinguisticTerms/WhatIsASimulfix.htm" ;
          
          rdfs:comment "A simulfix is a change or replacement of vowels or consonants (usually vowels) which changes the meaning of a word, e.g. \"eat\" in past tense becomes \"ate \"tooth\" becomes \"teeth\" when plural. [http://www-01.sil.org/linguistics/GlossaryOflinguisticTerms/WhatIsASimulfix.htm]"@en ,
                       """Also known as replacive morph: 
A replacive morph is a descriptive construct representing an internal modification.
Delimitation and History:
The replacive morph is a construct of taxonomic structuralism.
[Christian Lehmann, under \"replacive morph\" at http://linguistik.uni-erfurt.de:8080/lido/Lido]"""@en ;
          
          :example "In ‚man - men’, the latter contains the replacive morph ‚a -> e’. [Christian Lehmann, under \"replacive morph\" at http://linguistik.uni-erfurt.de:8080/lido/Lido]"@en .



###  http://mmoon.org/mmoon/Stem

:Stem rdf:type owl:Class ;
      
      rdfs:label "Stem"@en ;
      
      owl:equivalentClass gold:Stem ;
      
      rdfs:subClassOf :Morph ;
      
      rdfs:comment """In a word-form: The stem is the morph to which inflectional marking applies. It is the morphological representative of the lexeme in a given word-form and is specified for part of speech.

In a derived word: The stem is the morphological representative of the lexical basis from which it is derived. 

In a compound word: The stem is the morphological representative of one of the two stems the word is composed of."""@en .



###  http://mmoon.org/mmoon/Suffix

:Suffix rdf:type owl:Class ;
        
        rdfs:label "Suffix"@en ;
        
        owl:equivalentClass gold:Suffix ;
        
        rdfs:subClassOf :Affix ;
        
        rdfs:comment "A suffix is an affix that follows its stem or root. [Christian Lehmann, under \"suffix\" at http://linguistik.uni-erfurt.de:8080/lido/Lido ]"@en .



###  http://mmoon.org/mmoon/SyntheticWordform

:SyntheticWordform rdf:type owl:Class ;
                   
                   rdfs:label "Synthetic word-form"@en ;
                   
                   rdfs:subClassOf :Wordform ;
                   
                   rdfs:comment "A word form is synthetic 1 iff it is not analytic [i.e. all its semantic and grammatical components are represented in one word form]. [Christian Lehmann, under \"synthesis\" at http://linguistik.uni-erfurt.de:8080/lido/Lido]"@en ;
                   
                   :example "«went» is a synthetic word-form of the lexeme «go»."@en .



###  http://mmoon.org/mmoon/Transfix

:Transfix rdf:type owl:Class ;
          
          rdfs:label "Transfix"@en ;
          
          rdfs:subClassOf :Affix ;
          
          rdfs:comment "A transfix is a discontinuous affix at least one of whose components is an infix.  [Christian Lehmann, under \"transfix\" at http://linguistik.uni-erfurt.de:8080/lido/Lido ]"@en .



###  http://mmoon.org/mmoon/VerbalAdjective

:VerbalAdjective rdf:type owl:Class ;
                 
                 rdfs:label "Verbal adjective"@en ;
                 
                 rdfs:subClassOf :Conversion ;
                 
                 :example "German: \"regierend\"(VParticiple) 'to reign' --> \"regierend\"(Adj) 'reigning'."@de ;
                 
                 rdfs:comment "A verbal adjective is an adjective which is fomed by conversion from a verb and which entails no further derivational meaning except the entailed wordclass-change."@en .



###  http://mmoon.org/mmoon/VerbalCompound

:VerbalCompound rdf:type owl:Class ;
                
                rdfs:label "Verbal compound"@en ;
                
                rdfs:subClassOf :Compounding ;
                
                rdfs:comment "A verbal compound is a verb formed by composition of a verbal stem and another stem."@en ;
                
                :example "Eng.: \"force feed\"(V) = \"force\"(N) + \"feed\"(V)."@en .



###  http://mmoon.org/mmoon/VerbalInflection

:VerbalInflection rdf:type owl:Class ;
                  
                  rdfs:label "Verbal inflection"@en ;
                  
                  rdfs:subClassOf :Inflection ;
                  
                  rdfs:comment "Is the process of generating word-forms of verbal stems."@en .



###  http://mmoon.org/mmoon/VerbalNoun

:VerbalNoun rdf:type owl:Class ;
            
            rdfs:label "Verbal noun"@en ;
            
            rdfs:subClassOf :Conversion ;
            
            rdfs:comment "A verbal noun is a noun which is fomed by conversion from a verb and which entails no further derivational meaning except the entailed wordclass-change."@en ;
            
            :example "Engl.: \"to call\"(V) --> \"the call\"(N)."@en .



###  http://mmoon.org/mmoon/Word

:Word rdf:type owl:Class ;
      
      rdfs:label "Word"@en ;
      
      rdfs:subClassOf [ rdf:type owl:Restriction ;
                        owl:onProperty :hasRepresentation ;
                        owl:someValuesFrom :Representation
                      ] ;
      
      rdfs:comment """A word is a unit which is a constituent at the phrase level and above. It is sometimes identifiable according to such criteria as a) being the minimal possible unit in a reply, b) having features such as a regular stress pattern, and phonological changes conditioned by or blocked at word boundaries, c) being the largest unit resistant to insertion of new constituents within its boundaries, or d)  being the smallest constituent that can be moved within a sentence without making the sentence ungrammatical.
A word is sometimes placed, in a hierarchy of grammatical constituents, above the morpheme level and below the phrase level. [http://www-01.sil.org/linguistics/GlossaryOflinguisticTerms/WhatIsAWord.htm]"""@en ;
      
      rdfs:seeAlso """Christian Lehmann, under \"word\" at http://linguistik.uni-erfurt.de:8080/lido/Lido :
A word is a (grammatical) unit that enjoys a moderate degree of autonomy. I.e. while its parts tend to occupy fixed (morphological) positions, to be welded phonologically, to contract well-defined paradigmatic relations, all this is true to a lesser extent for the word itself and to an even lesser extent for the syntagm.
The cognitive counterpart of a word in general is a mental representation."""@en .



###  http://mmoon.org/mmoon/WordFormation

:WordFormation rdf:type owl:Class ;
               
               rdfs:label "Word-formation"@en ;
               
               rdfs:subClassOf :MorphologicalRelationship ;
               
               rdfs:seeAlso """Christian Lehmann, under \"word formation\" at http://linguistik.uni-erfurt.de:8080/lido/Lido :
Stem formation is the lexical part of morphology.
Stem formation is the formation of stems, normally on the basis of at least one component stem. Each stem thus generated potentially constitutes a lexeme [lexema] of its own."""@en ;
               
               rdfs:comment """Is the formation of words based on other words by the means of derivation and compounding. 

Word-formation is also called lexeme-formation and stem-formation ."""@en .



###  http://mmoon.org/mmoon/Wordform

:Wordform rdf:type owl:Class ;
          
          rdfs:label "Word-form"@en ;
          
          rdfs:subClassOf :Word ,
                          [ rdf:type owl:Restriction ;
                            owl:onProperty :consistsOfMorph ;
                            owl:someValuesFrom :Stem
                          ] ,
                          [ rdf:type owl:Restriction ;
                            owl:onProperty :inflectionalRelation ;
                            owl:someValuesFrom :Inflection
                          ] ;
          
          rdfs:comment """A word form is one of the morphological manifestations of a lexeme in text. For all parts of speech that inflect, the specification of inflectional categories for a lexeme generates the set of its word forms. [Christian Lehmann, under \"word form\" at http://linguistik.uni-erfurt.de:8080/lido/Lido]

It expresses the combination of a lexeme and a set of grammatical meanings. A word-form always is an inflectional variant of a lexeme."""@en ;
          
          :usageNote "The word-form is specified for the stem to which the inflectional or agreement markings apply and for the inflectional and agreement affixes which are involved by using the property :consistsOfMorph, thus explicating the morphs which are involved in the inflectional pattern of the word-form."@en ;
          
          :example "«said» is a word form of «say». [Christian Lehmann, under \"word form\" at http://linguistik.uni-erfurt.de:8080/lido/Lido]"@en .



###  http://mmoon.org/mmoon/ZeroMorph

:ZeroMorph rdf:type owl:Class ;
           
           rdfs:label "Zero morph"@en ;
           
           rdfs:subClassOf :Affix ,
                           [ rdf:type owl:Restriction ;
                             owl:onProperty :isAllomorphTo ;
                             owl:someValuesFrom :Morph
                           ] ;
           
           rdfs:comment """A morpheme that has a morphological meaning that corresponds to no overt form.  [Haspelmath and Sims: Understanding morphology. 2002:64]

A zero morpheme is a morpheme which has no significans. [Christian Lehmann, under \"zero morpheme\" at http://linguistik.uni-erfurt.de:8080/lido/Lido]"""@en ;
           
           :usageNote "A zero morpheme is posited only if it is in equipollent opposition to overt morphemes. If the term in question is, instead, the unmarked member of a privative opposition, no morpheme is posited. Conversion  can be conceived as derivation using a zero morpheme.  [Christian Lehmann, under \"zero morpheme\" at http://linguistik.uni-erfurt.de:8080/lido/Lido]"@en .



###  http://purl.org/linguistics/gold/Affix

gold:Affix rdf:type owl:Class .



###  http://purl.org/linguistics/gold/Circumfix

gold:Circumfix rdf:type owl:Class .



###  http://purl.org/linguistics/gold/Compound

gold:Compound rdf:type owl:Class .



###  http://purl.org/linguistics/gold/Infix

gold:Infix rdf:type owl:Class .



###  http://purl.org/linguistics/gold/LexicalItem

gold:LexicalItem rdf:type owl:Class .



###  http://purl.org/linguistics/gold/Prefix

gold:Prefix rdf:type owl:Class .



###  http://purl.org/linguistics/gold/Root

gold:Root rdf:type owl:Class .



###  http://purl.org/linguistics/gold/Stem

gold:Stem rdf:type owl:Class .



###  http://purl.org/linguistics/gold/Suffix

gold:Suffix rdf:type owl:Class .





#################################################################
#
#    Individuals
#
#################################################################


###  http://mmoon.org/mmoon/0

<http://mmoon.org/mmoon/0> rdf:type owl:NamedIndividual .




###  Generated by the OWL API (version 3.5.1) http://owlapi.sourceforge.net

