@prefix : <http://mmoon.org/mmoon/> .
@prefix dc: <http://purl.org/dc/elements/1.1/> .
@prefix owl: <http://www.w3.org/2002/07/owl#> .
@prefix rdf: <http://www.w3.org/1999/02/22-rdf-syntax-ns#> .
@prefix xml: <http://www.w3.org/XML/1998/namespace> .
@prefix xsd: <http://www.w3.org/2001/XMLSchema#> .
@prefix gold: <http://purl.org/linguistics/gold/> .
@prefix rdfs: <http://www.w3.org/2000/01/rdf-schema#> .
@prefix lexvo: <http://lexvo.org/ontology#> .
@prefix mmoon: <http://mmoon.org/mmoon/> .
@base <http://mmoon.org/mmoon/> .

<http://mmoon.org/mmoon/> rdf:type owl:Ontology ;
                          
                          rdfs:label "Multilingual Morpheme Ontology"@en ;
                          
                          rdfs:comment """The Multilingual Morpheme Ontology (MMoOn) is  an ontological model that contains the vocabulary needed to describe the morphological elements, meanings and representations of natural languages. 

This is the reference ontology from which various language specific MMoOn Inventories can be derived."""@en ;
                          
                          owl:versionInfo "Version 1.0, 2016"@en .


#################################################################
#
#    Annotation properties
#
#################################################################


###  http://mmoon.org/mmoon/example

:example rdf:type owl:AnnotationProperty .





#################################################################
#
#    Object Properties
#
#################################################################


###  http://mmoon.org/mmoon/belongsToLexeme

:belongsToLexeme rdf:type owl:ObjectProperty ;
                 
                 rdfs:label "belongs to lexeme"@en ;
                 
                 rdfs:comment "This property states that a word-form resource belongs into the inflectional paradigm of a lexeme resource."@en ;
                 
                 rdfs:range :Lexeme ;
                 
                 rdfs:domain :Wordform .



###  http://mmoon.org/mmoon/belongsToWord

:belongsToWord rdf:type owl:ObjectProperty ;
               
               rdfs:label "belongs to word"@en ;
               
               rdfs:domain :Morph ;
               
               rdfs:range :Word .



###  http://mmoon.org/mmoon/consistsOfMorph

:consistsOfMorph rdf:type owl:ObjectProperty ;
                 
                 rdfs:label "consists of morph"@en ;
                 
                 rdfs:range :Morph ;
                 
                 rdfs:domain :Word .



###  http://mmoon.org/mmoon/consistsOfRoot

:consistsOfRoot rdf:type owl:ObjectProperty ;
                
                rdfs:label "consists of root"@en ;
                
                rdfs:domain :Base ,
                            :Root ;
                
                rdfs:range :Root ;
                
                rdfs:domain :Stem ,
                            :Word .



###  http://mmoon.org/mmoon/consistsOfWord

:consistsOfWord rdf:type owl:ObjectProperty ;
                
                rdfs:label "consists of word"@en ;
                
                rdfs:comment "This property states that an analytic word-form (such as \"more big\" being the comparative form of the adjective \"big\") consists of of other word resources."@en ;
                
                rdfs:domain :AnalyticWordform ;
                
                rdfs:range :Word .



###  http://mmoon.org/mmoon/hasMeaning

:hasMeaning rdf:type owl:ObjectProperty ;
            
            rdfs:range :Meaning ;
            
            rdfs:domain :Morph ,
                        :Word .



###  http://mmoon.org/mmoon/hasMorphemicEntry

:hasMorphemicEntry rdf:type owl:ObjectProperty ;
                   
                   rdfs:label "has morphemic entry"@en ;
                   
                   rdfs:comment "This property states that a morpheme inventory resource has morphemes as morphemic entries, thus building the intension of the morpheme inventory."@en ;
                   
                   rdfs:range :Morpheme ;
                   
                   rdfs:domain :MorphemeInventory .



###  http://mmoon.org/mmoon/hasMorphologicalRelationship

:hasMorphologicalRelationship rdf:type owl:ObjectProperty ;
                              
                              rdfs:label "has morphological relationship"@en ;
                              
                              rdfs:comment "Specifies the morphological relationship of a word."@en ;
                              
                              rdfs:range :MorphologicalRelationship ;
                              
                              rdfs:domain :Word .



###  http://mmoon.org/mmoon/hasMorphosyntacticFeature

:hasMorphosyntacticFeature rdf:type owl:ObjectProperty .



###  http://mmoon.org/mmoon/hasRepresentation

:hasRepresentation rdf:type owl:ObjectProperty ;
                   
                   rdfs:label "has representation"@en ;
                   
                   rdfs:domain :Morph ;
                   
                   rdfs:range :Representation ;
                   
                   rdfs:domain :Word .



###  http://mmoon.org/mmoon/hasWordclassAffiliation

:hasWordclassAffiliation rdf:type owl:ObjectProperty ;
                         
                         rdfs:label "has wordclass affiliation"@en ;
                         
                         rdfs:domain :Morph ,
                                     :Word ;
                         
                         rdfs:range :WordclassAffiliation ;
                         
                         rdfs:subPropertyOf :hasMorphosyntacticFeature .



###  http://mmoon.org/mmoon/hasWordform

:hasWordform rdf:type owl:ObjectProperty ;
             
             rdfs:label "has wordform"@en ;
             
             rdfs:comment "This property states that (typically) a lexeme resource has and associated word-form resource."@en ;
             
             rdfs:domain :GrammaticalWord ,
                         :Lexeme ;
             
             rdfs:range :Wordform .



###  http://mmoon.org/mmoon/isDerivedFrom

:isDerivedFrom rdf:type owl:ObjectProperty ;
               
               rdfs:label "is derived from"@en ;
               
               rdfs:domain :GrammaticalWord ;
               
               rdfs:range :GrammaticalWord ;
               
               rdfs:domain :Lexeme ;
               
               rdfs:range :Lexeme .



###  http://purl.org/dc/elements/1.1/language

dc:language rdf:type owl:ObjectProperty ;
            
            rdfs:label "language"@en ;
            
            rdfs:range lexvo:Language ;
            
            rdfs:domain :MorphemeInventory .





#################################################################
#
#    Classes
#
#################################################################


###  http://lexvo.org/ontology#Language

lexvo:Language rdf:type owl:Class ;
               
               rdfs:label "Language"@en ;
               
               rdfs:isDefinedBy "http://lexvo.org/ontology#Language"@en .



###  http://mmoon.org/mmoon/ActionNoun

:ActionNoun rdf:type owl:Class ;
            
            rdfs:label "Action noun"@en ;
            
            rdfs:subClassOf :DeverbalNoun ;
            
            rdfs:comment "An action noun is a non-oriented verbal noun (nomen substantivum), i.e. one which designates the same kind of thing as a (finite) verb, viz. a situation core, except that this is hypostatized as an entity. [Christian Lehmann, under \"action noun\" at http://linguistik.uni-erfurt.de:8080/lido/Lido]"@en ;
            
            :example "Eng. \"to arrive\"(V) --> \"arrival\"(N)."@en .



###  http://mmoon.org/mmoon/AdjectivalInflection

:AdjectivalInflection rdf:type owl:Class ;
                      
                      rdfs:label "Adjectival inflection"@en ;
                      
                      rdfs:subClassOf :Inflection ;
                      
                      rdfs:comment "Is the process of generating word-forms of adjectival stems."@en .



###  http://mmoon.org/mmoon/AdjectiveCompound

:AdjectiveCompound rdf:type owl:Class ;
                   
                   rdfs:label "Adjective compound"@en ;
                   
                   rdfs:subClassOf :Compounding ;
                   
                   rdfs:comment "An adjective compound is an adjective formed by composition of an adjective stem and another stem."@en ;
                   
                   :example "Eng.: \"man-eating\"(Adj) = \"man\"(N) + \"eating\"(Adj)."@en .



###  http://mmoon.org/mmoon/AdjectiveNoun

:AdjectiveNoun rdf:type owl:Class ;
               
               rdfs:label "Adjective noun"@en ;
               
               rdfs:subClassOf :Conversion ;
               
               rdfs:comment "An adjective noun is a noun which is fomed by conversion from an adjective and which entails no further derivational meaning except the entailed wordclass-change."@en ;
               
               :example "Engl.: \"old\"(Adj) --> \"the old\"(N)."@en .



###  http://mmoon.org/mmoon/AdjectiveVerb

:AdjectiveVerb rdf:type owl:Class ;
               
               rdfs:label "Adjective verb"@en ;
               
               rdfs:subClassOf :Conversion ;
               
               :example "German: \"dicht\"(Adj.) 'impermeable' --> \"dichten\"(V) 'seal'."@de ;
               
               rdfs:comment "An adjective verb is a verb which is fomed by conversion from an adjective and which entails no further derivational meaning except the entailed wordclass-change."@en .



###  http://mmoon.org/mmoon/AdverbCompound

:AdverbCompound rdf:type owl:Class ;
                
                rdfs:label "Adverb compound"@en ;
                
                rdfs:subClassOf :Compounding ;
                
                rdfs:comment "An adverb compound is an adverb formed by composition of an adverb stem and another stem."@en ;
                
                :example "Eng.: \"downstream\"(Adv) = \"down\"(Adv) + \"stream\"(N)."@en .



###  http://mmoon.org/mmoon/AgentNominalizer

:AgentNominalizer rdf:type owl:Class ;
                  
                  rdfs:label "Agent nominalizer"@en ;
                  
                  rdfs:subClassOf :SemanticDerivation ;
                  
                  rdfs:comment "An agent nominalizer is a nominalizer which derives agent nouns. [Christian Lehmann, under \"agent nominalizer\" at http://linguistik.uni-erfurt.de:8080/lido/Lido]"@en ;
                  
                  :example "Engl. \"drive\" --> \"driver\""@en .



###  http://mmoon.org/mmoon/AgentNoun

:AgentNoun rdf:type owl:Class ;
           
           rdfs:label "Agent noun"@en ;
           
           rdfs:subClassOf :DeverbalNoun ;
           
           rdfs:comment "A noun which is derived from a verb base denoting someone or something that performs the action of the verb base."@en ;
           
           :example "Eng. \"to work\"(V) --> \"worker\"(N)."@en .



###  http://mmoon.org/mmoon/AnalyticWordform

:AnalyticWordform rdf:type owl:Class ;
                  
                  rdfs:label "Analytic word-form"@en ;
                  
                  rdfs:subClassOf :Wordform ;
                  
                  rdfs:comment """A word form is analytic iff it consists of more than one word form such that the lexical meaning provides the root of one of them, while the grammatical meaning components are coded in the other word forms (some of them possibly in the lexical word form).
An inflection is analytic to the extent that it consists of analytic word forms.

Delimitation and History:
’analytic’ is extensionally equivalent to ‚periphrastic’, but is also used to characterize a whole language type.
An analytic system has grammatical words; an isolating system does not.

Periphrastic conjugation is the formation of a verbal inflectional paradigm which consists of periphrastic forms.
Periphrastic conjugation is the formation of a verbal inflectional paradigm which consists of periphrastic forms.

Periphrasis is the combination of a grammatical word G with a lexical word L such that the result is equivalent to a morphological form of L inflected for the category of G.

Analytic Procedures:
Within one language, periphrasis is recognized by a paradigmatic relation between a periphrastic and a synthetic expression. Across languages or stages of one language, periphrasis in a looser sense is recognized on the basis of functional similarity. [Christian Lehmann, under \"analytic structure\" at http://linguistik.uni-erfurt.de:8080/lido/Lido]"""@en ;
                  
                  :example """The comparison of adjectives in English involves both inflectional forms (e.g. bigger) and periphrastic constructions (e.g. more interesting).
Engl. sang (synthetic) vs. has sung (periphrastic). [Christian Lehmann, under \"periphrasis\" at http://linguistik.uni-erfurt.de:8080/lido/Lido]"""@en .



###  http://mmoon.org/mmoon/ApplicativeVerb

:ApplicativeVerb rdf:type owl:Class ;
                 
                 rdfs:label "Applicative verb"@en ;
                 
                 rdfs:subClassOf :DeverbalVerb ;
                 
                 :example "German: \"steigen\"(V) 'rise' --> \"besteigen\"(V) 'climb'."@de ;
                 
                 rdfs:comment """An applicative verb is a derived transitive verb whose direct object has been promoted to this function from a more peripheral syntactic function that it has with the base verb.

The base may be transitive, in which case its direct object is demoted upon the derivation of the applicative verb.
[Christian Lehmann, under \"applicative verb\" at http://linguistik.uni-erfurt.de:8080/lido/Lido]"""@en .



###  http://mmoon.org/mmoon/AugmentativeNoun

:AugmentativeNoun rdf:type owl:Class ;
                  
                  rdfs:label "Augmentative noun"@en ;
                  
                  rdfs:subClassOf :DenominalNoun ;
                  
                  rdfs:seeAlso "http://purl.org/olia/olia.owl#Augmentative" ,
                               "http://purl.org/linguistics/gold/AugmentativeSize" ;
                  
                  rdfs:comment "A noun which is derived from a noun base that denotes big or large size. Possible connotations include strong, imposing, ugly."@en ,
                               """Augmentation is the derivational modification of a noun by the concept „big, large“. Possible connotations include „strong, imposing, ugly“.
A noun is augmentative 1 iff it is derived by augmentation. [Christian Lehmann, under \"augmentation\" at http://linguistik.uni-erfurt.de:8080/lido/Lido]"""@en .



###  http://mmoon.org/mmoon/Base

:Base rdf:type owl:Class .



###  http://mmoon.org/mmoon/CausativeVerb

:CausativeVerb rdf:type owl:Class ;
               
               rdfs:label "Causative verb"@en ;
               
               rdfs:subClassOf :DeverbalVerb ;
               
               rdfs:comment """A causative verb is an n-place verb (with n > 1) which is derived from an n-1-place verb in such a way that the additional semantic slot is mapped onto the subject slot and is occupied by a superordinate agent which causes the situation designated by the base.

An underived verb cannot be causative by this definition. However, the paradigmatic lexical relation of Engl. «kill» to «die» may be called ‚semantically causative’. [Christian Lehmann, under \"causative verb\" at http://linguistik.uni-erfurt.de:8080/lido/Lido]"""@en ;
               
               :example """Eng.: \"fall\"(V) --> \"fell\"(V).
[Christian Lehmann, under \"causative verb\" at http://linguistik.uni-erfurt.de:8080/lido/Lido]"""@en .



###  http://mmoon.org/mmoon/CollectivePersonNoun

:CollectivePersonNoun rdf:type owl:Class ;
                      
                      rdfs:label "Collective person noun"@en ;
                      
                      rdfs:subClassOf :DenominalNoun ;
                      
                      :example "German: \"Lehrer\"(N) 'teacher' --> \"Lehrerschaft\"(N) 'body of teachers'."@de ;
                      
                      rdfs:comment "A noun which is derived from a noun base that denotes group of persons."@en .



###  http://mmoon.org/mmoon/CompoundWord

:CompoundWord rdf:type owl:Class ;
              
              rdfs:label "Compound Word"@en ;
              
              owl:equivalentClass gold:Compound ;
              
              rdfs:subClassOf :Lexeme ,
                              [ rdf:type owl:Restriction ;
                                owl:onProperty :hasMorphologicalRelationship ;
                                owl:onClass :Compounding ;
                                owl:qualifiedCardinality "1"^^xsd:nonNegativeInteger
                              ] ;
              
              rdfs:comment """A compound is a stem formed by composition. [Christian Lehmann, under \"compound\" at http://linguistik.uni-erfurt.de:8080/lido/Lido]

Is a kind of lexeme which is formed by the combination of two stems."""@en ;
              
              :example "Engl. \"playground\"."@en .



###  http://mmoon.org/mmoon/Compounding

:Compounding rdf:type owl:Class ;
             
             rdfs:label "Compounding"@en ;
             
             rdfs:subClassOf :WordFormation ;
             
             rdfs:comment """Compounding [compositio thematum] is the formation of a stem by combination of two stems. Both stems may already be complex.[Christian Lehmann, under \"compounding\" at http://linguistik.uni-erfurt.de:8080/lido/Lido]

Compounds, in English and some other languages, can be written as one word or two separate words, and they can be hyphenated as well. [http://www.glottopedia.org/index.php/Compound]

Is the process of lexeme-formation by combining two stems."""@en .



###  http://mmoon.org/mmoon/Conjugation

:Conjugation rdf:type owl:Class ;
             
             rdfs:label "Conjugation"@en ;
             
             rdfs:subClassOf :VerbalInflection ;
             
             rdfs:comment "Is the inflection of a verb. Conjugation categories commonly include person, number, gender, aspect, tense, mood, voice and non-finite subcategories. [Christian Lehmann, under \"conjugation\" at http://linguistik.uni-erfurt.de:8080/lido/Lido ]"@en .



###  http://mmoon.org/mmoon/Conversion

:Conversion rdf:type owl:Class ;
            
            rdfs:label "Conversion"@en ;
            
            rdfs:subClassOf :Derivation ;
            
            rdfs:comment """Conversion, also called zero-derivation, is the formation of a lexeme from another part of speech which entails no further derivational meaning except that which is entailed in the wordclass-change. All other derivations which include an affix marking the wordclass-change but also do not entail further derivational meaning belong into the according mmoon:Derived[Wordclass] subclasses.

In morphology, conversion is a process which derives words without changing the phonological shape of the base. [http://www.glottopedia.org/index.php/Conversion]

Conversion [recategorizatio] is the implicit change of the word class of a stem.
Conversion [recategorizatio] is not a kind of derivation 1 if the latter is conceived as involving a morphological process. At the level of formal representation, however, conversion [recategorizatio] may be conceived as dependency of a stem on a zero affix.  [Christian Lehmann, under \"conversion\" at http://linguistik.uni-erfurt.de:8080/lido/Lido]"""@en .



###  http://mmoon.org/mmoon/DeadjectivalAdjective

:DeadjectivalAdjective rdf:type owl:Class ;
                       
                       rdfs:label "Deadjectival adjective"@en ;
                       
                       rdfs:subClassOf :DerivedAdjective ;
                       
                       rdfs:comment "Is an adjective which derived from an adjective base."@en .



###  http://mmoon.org/mmoon/DeadjectivalAdverb

:DeadjectivalAdverb rdf:type owl:Class ;
                    
                    rdfs:label "DeadjectivalAdverb"@en ;
                    
                    rdfs:subClassOf :DerivedAdverb ;
                    
                    rdfs:comment """Is an adverb which derived from an adjective base.

Add instance here, if the language of the given morpheme inventory exhibits affixal marking for word-class change but adds NO further derivational meaning(s). For all derived lexemes that consist of a derivational affix denoting some additional meaning, the respective subclass must be instantiated or newly created."""@en .



###  http://mmoon.org/mmoon/DeadjectivalNoun

:DeadjectivalNoun rdf:type owl:Class ;
                  
                  rdfs:label "Deadjectival noun"@en ;
                  
                  rdfs:subClassOf :DerivedNoun ;
                  
                  rdfs:comment """Is a noun which derived from an adjective base.

Add instance here, if the language of the given morpheme inventory exhibits affixal marking for word-class change but adds NO further derivational meaning(s). For all derived lexemes that consist of a derivational affix denoting some additional meaning, the respective subclass must be instantiated or newly created."""@en .



###  http://mmoon.org/mmoon/DeadjectivalVerb

:DeadjectivalVerb rdf:type owl:Class ;
                  
                  rdfs:label "Deadjectival verb"@en ;
                  
                  rdfs:subClassOf :DerivedVerb ;
                  
                  rdfs:comment """Is a verb which derived from an adjective base.

Add instance here, if the language of the given morpheme inventory exhibits affixal marking for word-class change but adds NO further derivational meaning(s). For all derived lexemes that consist of a derivational affix denoting some additional meaning, the respective subclass must be instantiated or newly created."""@en .



###  http://mmoon.org/mmoon/DeadverbalAdverb

:DeadverbalAdverb rdf:type owl:Class ;
                  
                  rdfs:label "Deadverbal adverb"@en ;
                  
                  rdfs:subClassOf :DerivedAdverb ;
                  
                  rdfs:comment "Is an adverb which derived from an adverb base."@en .



###  http://mmoon.org/mmoon/Declension

:Declension rdf:type owl:Class ;
            
            rdfs:label "Declension"@en ;
            
            rdfs:subClassOf :NominalInflection ;
            
            rdfs:comment "Is the inflection of a noun. Relevant categories commonly include gender, number, case, possessive and definiteness. [Christian Lehmann, under \"declension\" at http://linguistik.uni-erfurt.de:8080/lido/Lido ]"@en .



###  http://mmoon.org/mmoon/Degree

:Degree rdf:type owl:Class ;
        
        rdfs:label "Degree"@en ;
        
        rdfs:subClassOf :AdjectivalInflection ;
        
        rdfs:comment "Attributively used adjectives inflect for the category degree of comparison. In agreement with the noun it modifies they can also be marked for nominal inflectional categories such as gender, case and number."@en .



###  http://mmoon.org/mmoon/DenominalAdjective

:DenominalAdjective rdf:type owl:Class ;
                    
                    rdfs:label "Denominal adjective"@en ;
                    
                    rdfs:subClassOf :DerivedAdjective ;
                    
                    rdfs:comment """Is an adjective which derived from a noun base.

Add instance here, if the language of the given morpheme inventory exhibits affixal marking for word-class change but adds NO further derivational meaning(s). For all derived lexemes that consist of a derivational affix denoting some additional meaning, the respective subclass must be instantiated or newly created."""@en .



###  http://mmoon.org/mmoon/DenominalAdverb

:DenominalAdverb rdf:type owl:Class ;
                 
                 rdfs:label "Denominal adverb"@en ;
                 
                 rdfs:subClassOf :DerivedAdverb ;
                 
                 rdfs:comment """Is an adverb which derived from a noun base.

Add instance here, if the language of the given morpheme inventory exhibits affixal marking for word-class change but adds NO further derivational meaning(s). For all derived lexemes that consist of a derivational affix denoting some additional meaning, the respective subclass must be instantiated or newly created."""@en .



###  http://mmoon.org/mmoon/DenominalNoun

:DenominalNoun rdf:type owl:Class ;
               
               rdfs:label "Denominal noun"@en ;
               
               rdfs:subClassOf :DerivedNoun ;
               
               rdfs:comment "Is a noun which derived from a noun base."@en .



###  http://mmoon.org/mmoon/DenominalVerb

:DenominalVerb rdf:type owl:Class ;
               
               rdfs:label "Denominal verb"@en ;
               
               rdfs:subClassOf :DerivedVerb ;
               
               rdfs:comment """Is a verb which derived from a noun base.

Add instance here, if the language of the given morpheme inventory exhibits affixal marking for word-class change but adds NO further derivational meaning(s). For all derived lexemes that consist of a derivational affix denoting some additional meaning, the respective subclass must be instantiated or newly created."""@en .



###  http://mmoon.org/mmoon/Derivation

:Derivation rdf:type owl:Class ;
            
            rdfs:label "Derivation"@en ;
            
            rdfs:subClassOf :WordFormation ;
            
            rdfs:comment "Is the process of lexeme-formation which is morphologically conditioned and involves the modification of a base."@en .



###  http://mmoon.org/mmoon/DerivedAdjective

:DerivedAdjective rdf:type owl:Class ;
                  
                  rdfs:label "Derived adjective"@en ;
                  
                  rdfs:subClassOf :Derivation ;
                  
                  rdfs:comment "Is an adjective which derived from a base."@en .



###  http://mmoon.org/mmoon/DerivedAdverb

:DerivedAdverb rdf:type owl:Class ;
               
               rdfs:label "Derived adverb"@en ;
               
               rdfs:subClassOf :Derivation ;
               
               rdfs:comment "Is an adverb which derived from a base."@en .



###  http://mmoon.org/mmoon/DerivedNoun

:DerivedNoun rdf:type owl:Class ;
             
             rdfs:label "Derived noun"@en ;
             
             rdfs:subClassOf :Derivation ;
             
             rdfs:comment "Is a noun which derived from a base."@en .



###  http://mmoon.org/mmoon/DerivedVerb

:DerivedVerb rdf:type owl:Class ;
             
             rdfs:label "Derived verb"@en ;
             
             rdfs:subClassOf :Derivation ;
             
             rdfs:comment "Is a verb which derived from a base."@en .



###  http://mmoon.org/mmoon/DerivedWord

:DerivedWord rdf:type owl:Class ;
             
             rdfs:label "Derived word"@en ;
             
             rdfs:subClassOf :Lexeme ,
                             [ rdf:type owl:Restriction ;
                               owl:onProperty :hasMorphologicalRelationship ;
                               owl:onClass :Derivation ;
                               owl:qualifiedCardinality "1"^^xsd:nonNegativeInteger
                             ] ;
             
             :example "\"replay\" is a derived word from the lexeme \"play\"."@en ;
             
             rdfs:comment """A derivate is a stem generated by derivation [derivatio]. [Christian Lehmann, under \"derivate\" at http://linguistik.uni-erfurt.de:8080/lido/Lido]

Is a kind of lexeme which is formed by the morphological modification of a base."""@en .



###  http://mmoon.org/mmoon/DesiderativeVerb

:DesiderativeVerb rdf:type owl:Class ;
                  
                  rdfs:label "Desiderative verb"@en ;
                  
                  rdfs:subClassOf :DeverbalVerb ;
                  
                  rdfs:comment "A verb which is derived from a verb base denoting to want the meaning of the verb base."@en ;
                  
                  :example "Sanskrit: \"‚s:r.no-ti\" (V) 'hears' --> \"‚su-’sr¡u-.sa-ti\"(V) (RED-hear-DES-3.SG) 'wants to hear'."@sa .



###  http://mmoon.org/mmoon/DeverbalAdjective

:DeverbalAdjective rdf:type owl:Class ;
                   
                   rdfs:label "Deverbal Adjective"@en ;
                   
                   rdfs:subClassOf :DerivedAdjective ;
                   
                   rdfs:comment """Is an adjective which derived from a verb base.

Add instance here, if the language of the given morpheme inventory exhibits affixal marking for word-class change but adds NO further derivational meaning(s). For all derived lexemes that consist of a derivational affix denoting some additional meaning, the respective subclass must be instantiated or newly created."""@en .



###  http://mmoon.org/mmoon/DeverbalAdverb

:DeverbalAdverb rdf:type owl:Class ;
                
                rdfs:label "Deverbal adverb"@en ;
                
                rdfs:subClassOf :DerivedAdverb ;
                
                rdfs:comment """Is an adverb which derived from a verb base.

Add instance here, if the language of the given morpheme inventory exhibits affixal marking for word-class change but adds NO further derivational meaning(s). For all derived lexemes that consist of a derivational affix denoting some additional meaning, the respective subclass must be instantiated or newly created."""@en .



###  http://mmoon.org/mmoon/DeverbalNoun

:DeverbalNoun rdf:type owl:Class ;
              
              rdfs:label "Deverbal noun"@en ;
              
              rdfs:subClassOf :DerivedNoun ;
              
              rdfs:comment """Is a noun which derived from a verb base.

Add instance here, if the language of the given morpheme inventory exhibits affixal marking for word-class change but adds NO further derivational meaning(s). For all derived lexemes that consist of a derivational affix denoting some additional meaning, the respective subclass must be instantiated or newly created."""@en .



###  http://mmoon.org/mmoon/DeverbalVerb

:DeverbalVerb rdf:type owl:Class ;
              
              rdfs:label "Deverbal verb"@en ;
              
              rdfs:subClassOf :DerivedVerb ;
              
              rdfs:comment "Is a verb which derived from a verb base."@en .



###  http://mmoon.org/mmoon/DiminutiveAdjective

:DiminutiveAdjective rdf:type owl:Class ;
                     
                     rdfs:label "Diminutive adjective"@en ;
                     
                     rdfs:subClassOf :DeadjectivalAdjective ;
                     
                     rdfs:seeAlso "http://purl.org/linguistics/gold/DiminuativeSize" ;
                     
                     rdfs:comment "An adjective which is derived from an adjective base that denotes a smaller intensity than the adjective base."@en ;
                     
                     :example "Eng. \"small\"(ADJ) --> \"smallish\"(ADJ)"@en .



###  http://mmoon.org/mmoon/DiminutiveNoun

:DiminutiveNoun rdf:type owl:Class ;
                
                rdfs:label "Diminutive noun"@en ;
                
                rdfs:subClassOf :DenominalNoun ;
                
                :example "German \"Kind\"(N) --> \"Kindchen\"(N)"@de ,
                         "Eng. \"duck\"(N) --> \"duckling\"(N)"@en ;
                
                rdfs:seeAlso "http://purl.org/linguistics/gold/DiminuativeSize" ;
                
                rdfs:comment "A noun which is derived from a noun base that denotes endearment, small size or small intensity."@en ;
                
                rdfs:seeAlso <http://purl.org/olia/olia.owl#DiminutiveNoun> .



###  http://mmoon.org/mmoon/FactitiveVerb

:FactitiveVerb rdf:type owl:Class ;
               
               rdfs:label "Factitive verb"@en ;
               
               rdfs:subClassOf :DeadjectivalVerb ;
               
               :example """German: \"tot\"(Adj) 'dead' --> \"töten\"(V) 'to kill'.
 [Christian Lehmann, under \"factitive verb\" at http://linguistik.uni-erfurt.de:8080/lido/Lido]"""@de ;
               
               rdfs:comment """A factitive verb is a causative verb based on an adjective (or a stative intransitive verb).

Delimitation and History:
While there may be a subordinate agent in a causative construction, there may be none in a factitive one. This has sometimes been a reason for not subsuming factitive under causative. [Christian Lehmann, under \"factitive verb\" at http://linguistik.uni-erfurt.de:8080/lido/Lido]"""@en ;
               
               :example """Engl.:\"black\"(Adj) --> \"blacken\"(Vtr.).
 [Christian Lehmann, under \"factitive verb\" at http://linguistik.uni-erfurt.de:8080/lido/Lido]"""@en .



###  http://mmoon.org/mmoon/FemaleNoun

:FemaleNoun rdf:type owl:Class ;
            
            rdfs:label "Female noun"@en ;
            
            rdfs:subClassOf :DenominalNoun ;
            
            :example "German: \"Fahrer\"(N) 'male driver' --> \"Fahrerin\"(N) 'female driver'."@de ;
            
            rdfs:comment "A noun which is derived from a noun base that denotes a female person."@en .



###  http://mmoon.org/mmoon/GrammaticalWord

:GrammaticalWord rdf:type owl:Class ;
                 
                 rdfs:label "Grammatical word"@en ;
                 
                 rdfs:subClassOf :Word ;
                 
                 rdfs:comment "A grammatical word is a word which is a grammatical formative. [Christian Lehmann, under \"grammatical word\" at http://linguistik.uni-erfurt.de:8080/lido/Lido]"@en ;
                 
                 :example "Engl. «be», «of».  [Christian Lehmann, under \"grammatical word\" at http://linguistik.uni-erfurt.de:8080/lido/Lido]"@en .



###  http://mmoon.org/mmoon/Inflection

:Inflection rdf:type owl:Class ;
            
            rdfs:label "Inflection"@en ;
            
            rdfs:subClassOf :MorphologicalRelationship ;
            
            rdfs:comment """Inflection [flexio] is the syntactically relevant part of morphology. It generates word forms (inflectional forms) of word stems.
In contrast to derivation, inflection  never results in a change of word class and produces a predictable, regular change of meaning (for regular word-forms only).
Its expression is typically located farther from the root than that of derivation. [Christian Lehmann, under \"inflection\" at http://linguistik.uni-erfurt.de:8080/lido/Lido]

Is the process of generating word-forms of lexical stems. This class can be extended to describe the inflectional classes of the lexemes of a language."""@en .



###  http://mmoon.org/mmoon/InstrumentNoun

:InstrumentNoun rdf:type owl:Class ;
                
                rdfs:label "Instrument noun"@en ;
                
                rdfs:subClassOf :DeverbalNoun ;
                
                :example "German: \"lenken\"(V) 'to steer'--> \"Lenker\"(N) 'handle-bar, steering wheel'. [Christian Lehmann, under \"instrument noun\" at http://linguistik.uni-erfurt.de:8080/lido/Lido]"@de ;
                
                rdfs:comment "An instrument noun is an oriented deverbal noun that designates something that functions as an instrument in the situation designated by the base verb. [Christian Lehmann, under \"instrument noun\" at http://linguistik.uni-erfurt.de:8080/lido/Lido]"@en .



###  http://mmoon.org/mmoon/Introflection

:Introflection rdf:type owl:Class ;
               
               rdfs:label "Introflection"@en ;
               
               rdfs:subClassOf :MorphologicalRelationship ;
               
               rdfs:comment "Nonconcatenative morphology, also called discontinuous morphology and introflection, is a form of word-formation [and inflection] in which the root is modified and does not involve stringing morphemes together. [Haspelmath and Sims: Understanding morphology. 2002, Sections 3.1.2 - 3.1.4]"@en .



###  http://mmoon.org/mmoon/IrregularConjugation

:IrregularConjugation rdf:type owl:Class ;
                      
                      rdfs:label "Irregular conjugation"@en ;
                      
                      rdfs:subClassOf :Conjugation ;
                      
                      rdfs:comment "Conjugation that deviates from the regular inflectional pattern."@en .



###  http://mmoon.org/mmoon/Lexeme

:Lexeme rdf:type owl:Class ;
        
        rdfs:label "Lexeme"@en ;
        
        owl:equivalentClass gold:LexicalItem ;
        
        rdfs:subClassOf :Word ,
                        [ rdf:type owl:Restriction ;
                          owl:onProperty :consistsOfMorph ;
                          owl:someValuesFrom :Root
                        ] ,
                        [ rdf:type owl:Restriction ;
                          owl:onProperty :consistsOfMorph ;
                          owl:someValuesFrom :Base
                        ] ;
        
        rdfs:comment """A lexeme [lexema] is a word in its capacity as a unit of the lexicon. In a text, it appears in form of diverse word forms. [Christian Lehmann, under \"lexeme\" at http://linguistik.uni-erfurt.de:8080/lido/Lido]

A lexeme is a word as it appears as an entry in a dictionary. It has a holistic abstract sense representing the core meaning shared by a set of closely-related word-forms. A lexeme can only be a word that inflects."""@en .



###  http://mmoon.org/mmoon/MaterialAdjective

:MaterialAdjective rdf:type owl:Class ;
                   
                   rdfs:label "Material adjective"@en ;
                   
                   rdfs:subClassOf :DenominalAdjective ;
                   
                   :example "German: Holz 'wood' --> hölzern 'wooden'."@de ;
                   
                   rdfs:comment "An adjective which is derived from a noun base denoting some kind of material and means 'being made of this material'."@en .



###  http://mmoon.org/mmoon/Meaning

:Meaning rdf:type owl:Class .



###  http://mmoon.org/mmoon/Morph

:Morph rdf:type owl:Class .



###  http://mmoon.org/mmoon/Morpheme

:Morpheme rdf:type owl:Class .



###  http://mmoon.org/mmoon/MorphemeInventory

:MorphemeInventory rdf:type owl:Class ;
                   
                   rdfs:label "Morpheme inventory"@en ;
                   
                   rdfs:comment "The morpheme inventory is the object that contains morphemic entries. It is specified for the natural language it describes."@en .



###  http://mmoon.org/mmoon/MorphologicalRelationship

:MorphologicalRelationship rdf:type owl:Class ;
                           
                           rdfs:label "Morphological Relationship"@en ;
                           
                           rdfs:comment """Is the relationship between word-forms of a lexeme (inflection) or the relationship between lexemes of a word family (derivation). [Haspelmath and Sims: Understanding morphology. 2002:18]

NOTE: In all subclasses of \"MorphologicalRelationship\" the semantic or grammatic categories are not specified. They only declare what kind of morphological relationship(s) is/are expressed on a word."""@en .



###  http://mmoon.org/mmoon/NoDegree

:NoDegree rdf:type owl:Class ;
          
          rdfs:label "No degree"@en ;
          
          rdfs:subClassOf :AdjectivalInflection ;
          
          rdfs:comment "Some adjectives do not inflect for the category degree of comparison, e.g. \"dead\", \"absolute\", \"pregnant\". In agreement with the noun it modifies it can still be marked for nominal inflectional categories such as gender, case and number."@en .



###  http://mmoon.org/mmoon/NoInflection

:NoInflection rdf:type owl:Class ;
              
              rdfs:label "No inflection"@en ;
              
              rdfs:subClassOf :MorphologicalRelationship ;
              
              rdfs:comment "This class marks words which do not inflect. This holds for most grammatical words but also for some lexemes (e.g. the invariable adjective \"super\" in German)."@en .



###  http://mmoon.org/mmoon/NominalAdverb

:NominalAdverb rdf:type owl:Class ;
               
               rdfs:label "Nominal adverb"@en ;
               
               rdfs:subClassOf :Conversion ;
               
               rdfs:comment "A nominal adverb is an adverb which is fomed by conversion from a noun and which entails no further derivational meaning except the entailed wordclass-change."@en ;
               
               :example "Engl.: \"backstage\"(N) --> \"backstage\"(Adv)."@en .



###  http://mmoon.org/mmoon/NominalCompound

:NominalCompound rdf:type owl:Class ;
                 
                 rdfs:label "Nominal compound"@en ;
                 
                 rdfs:subClassOf :Compounding ;
                 
                 rdfs:comment "A nominal compound is a noun formed by composition of a nominal stem and another stem."@en ;
                 
                 :example "Engl.: \"blackboard\"(N) = \"black\"(Adj) + \"board\"(N)."@en .



###  http://mmoon.org/mmoon/NominalInflection

:NominalInflection rdf:type owl:Class ;
                   
                   rdfs:label "Nominal inflection"@en ;
                   
                   rdfs:subClassOf :Inflection ;
                   
                   rdfs:comment "Is the process of generating word-forms of nominal stems."@en .



###  http://mmoon.org/mmoon/NominalVerb

:NominalVerb rdf:type owl:Class ;
             
             rdfs:label "Nominal verb"@en ;
             
             rdfs:subClassOf :Conversion ;
             
             rdfs:comment "A nominal verb is a verb which is fomed by conversion from a noun and which entails no further derivational meaning except the entailed wordclass-change."@en ;
             
             :example "Engl.: \"the steam\"(N) --> \"to steam\"(V)."@en .



###  http://mmoon.org/mmoon/NounAdjective

:NounAdjective rdf:type owl:Class ;
               
               rdfs:label "Noun adjective"@en ;
               
               rdfs:subClassOf :Conversion ;
               
               rdfs:comment "A noun adjective is an adjective which is fomed by conversion from a noun and which entails no further derivational meaning except the entailed wordclass-change."@en ;
               
               :example "Engl.: \"Swiss\"(NPr) --> \"Swiss\"(Adj)."@en .



###  http://mmoon.org/mmoon/PatientNoun

:PatientNoun rdf:type owl:Class ;
             
             rdfs:label "Patient noun"@en ;
             
             rdfs:subClassOf :DeverbalNoun ;
             
             :example "German: \"bestellen\"(V) 'to order' --> \"Bestellung\"(N) 'the thing you ordered'."@de ;
             
             rdfs:comment "A patient noun is an oriented verbal noun designating the undergoer of the verbal base. [Christian Lehmann, under \"patient noun\" at http://linguistik.uni-erfurt.de:8080/lido/Lido]"@en .



###  http://mmoon.org/mmoon/RegularConjugation

:RegularConjugation rdf:type owl:Class ;
                    
                    rdfs:label "Regular conjugation"@en ;
                    
                    rdfs:subClassOf :Conjugation ;
                    
                    rdfs:comment "Conjugation that exhibits a regular inflectional pattern."@en .



###  http://mmoon.org/mmoon/Representation

:Representation rdf:type owl:Class .



###  http://mmoon.org/mmoon/Root

:Root rdf:type owl:Class .



###  http://mmoon.org/mmoon/SemanticDerivation

:SemanticDerivation rdf:type owl:Class .



###  http://mmoon.org/mmoon/Stem

:Stem rdf:type owl:Class .



###  http://mmoon.org/mmoon/SyntheticWordform

:SyntheticWordform rdf:type owl:Class ;
                   
                   rdfs:label "Synthetic word-form"@en ;
                   
                   rdfs:subClassOf :Wordform ;
                   
                   rdfs:comment "A word form is synthetic 1 iff it is not analytic [i.e. all its semantic and grammatical components are represented in one word form]. [Christian Lehmann, under \"synthesis\" at http://linguistik.uni-erfurt.de:8080/lido/Lido]"@en ;
                   
                   :example "«went» is a synthetic word-form of the lexeme «go»."@en .



###  http://mmoon.org/mmoon/VerbalAdjective

:VerbalAdjective rdf:type owl:Class ;
                 
                 rdfs:label "Verbal adjective"@en ;
                 
                 rdfs:subClassOf :Conversion ;
                 
                 :example "German: \"regierend\"(VParticiple) 'to reign' --> \"regierend\"(Adj) 'reigning'."@de ;
                 
                 rdfs:comment "A verbal adjective is an adjective which is fomed by conversion from a verb and which entails no further derivational meaning except the entailed wordclass-change."@en .



###  http://mmoon.org/mmoon/VerbalCompound

:VerbalCompound rdf:type owl:Class ;
                
                rdfs:label "Verbal compound"@en ;
                
                rdfs:subClassOf :Compounding ;
                
                rdfs:comment "A verbal compound is a verb formed by composition of a verbal stem and another stem."@en ;
                
                :example "Eng.: \"force feed\"(V) = \"force\"(N) + \"feed\"(V)."@en .



###  http://mmoon.org/mmoon/VerbalInflection

:VerbalInflection rdf:type owl:Class ;
                  
                  rdfs:label "Verbal inflection"@en ;
                  
                  rdfs:subClassOf :Inflection ;
                  
                  rdfs:comment "Is the process of generating word-forms of verbal stems."@en .



###  http://mmoon.org/mmoon/VerbalNoun

:VerbalNoun rdf:type owl:Class ;
            
            rdfs:label "Verbal noun"@en ;
            
            rdfs:subClassOf :Conversion ;
            
            rdfs:comment "A verbal noun is a noun which is fomed by conversion from a verb and which entails no further derivational meaning except the entailed wordclass-change."@en ;
            
            :example "Engl.: \"to call\"(V) --> \"the call\"(N)."@en .



###  http://mmoon.org/mmoon/Word

:Word rdf:type owl:Class ;
      
      rdfs:label "Word"@en ;
      
      rdfs:comment """A word is a unit which is a constituent at the phrase level and above. It is sometimes identifiable according to such criteria as a) being the minimal possible unit in a reply, b) having features such as a regular stress pattern, and phonological changes conditioned by or blocked at word boundaries, c) being the largest unit resistant to insertion of new constituents within its boundaries, or d)  being the smallest constituent that can be moved within a sentence without making the sentence ungrammatical.
A word is sometimes placed, in a hierarchy of grammatical constituents, above the morpheme level and below the phrase level. [http://www-01.sil.org/linguistics/GlossaryOflinguisticTerms/WhatIsAWord.htm]

A word is a (grammatical) unit that enjoys a moderate degree of autonomy. I.e. while its parts tend to occupy fixed (morphological) positions, to be welded phonologically, to contract well-defined paradigmatic relations, all this is true to a lesser extent for the word itself and to an even lesser extent for the syntagm.
The cognitive counterpart of a word in general is a mental representation. [Christian Lehmann, under \"word\" at http://linguistik.uni-erfurt.de:8080/lido/Lido]"""@en .



###  http://mmoon.org/mmoon/WordFormation

:WordFormation rdf:type owl:Class ;
               
               rdfs:label "Word-formation"@en ;
               
               rdfs:subClassOf :MorphologicalRelationship ;
               
               rdfs:comment """Stem formation is the lexical part of morphology.
Stem formation is the formation of stems, normally on the basis of at least one component stem. Each stem thus generated potentially constitutes a lexeme [lexema] of its own.  [Christian Lehmann, under \"word formation\" at http://linguistik.uni-erfurt.de:8080/lido/Lido]"""@en .



###  http://mmoon.org/mmoon/WordclassAffiliation

:WordclassAffiliation rdf:type owl:Class .



###  http://mmoon.org/mmoon/Wordform

:Wordform rdf:type owl:Class ;
          
          rdfs:label "Word-form"@en ;
          
          rdfs:subClassOf :Word ,
                          [ rdf:type owl:Restriction ;
                            owl:onProperty :hasMorphologicalRelationship ;
                            owl:someValuesFrom :Inflection
                          ] ,
                          [ rdf:type owl:Restriction ;
                            owl:onProperty :consistsOfMorph ;
                            owl:someValuesFrom :Root
                          ] ,
                          [ rdf:type owl:Restriction ;
                            owl:onProperty :consistsOfMorph ;
                            owl:someValuesFrom :Stem
                          ] ;
          
          rdfs:comment """A word form is one of the morphological manifestations of a lexeme in text. For all parts of speech that inflect, the specification of inflectional categories for a lexeme generates the set of its word forms. [Christian Lehmann, under \"word form\" at http://linguistik.uni-erfurt.de:8080/lido/Lido]

It expresses the combination of a lexeme and a set of grammatical meanings. A word-form always is an inflectional variant of a lexeme."""@en ;
          
          :example "«said» is a word form of «say». [Christian Lehmann, under \"word form\" at http://linguistik.uni-erfurt.de:8080/lido/Lido]"@en .



###  http://purl.org/linguistics/gold/Compound

gold:Compound rdf:type owl:Class .



###  http://purl.org/linguistics/gold/LexicalItem

gold:LexicalItem rdf:type owl:Class .




###  Generated by the OWL API (version 3.5.0) http://owlapi.sourceforge.net

